Split up Facade.v into a bunch of files

src/GoExamples.v
@@ -1,10 +1,295 @@
 Require Import List String.
 Require Import StringMap.
-Require Import Go.
+Require Import Word Prog BasicProg Pred.
+Require Import GoSemantics GoHoare GoExtraction.
 Import ListNotations.
 Import Go.
 
 Local Open Scope string_scope.
+
+Example append_list_in_pair : sigT (fun p => forall (a x : nat) xs,
+  EXTRACT Ret (a, x :: xs)
+  {{ 0 ~> (a, xs) * 1 ~> x }}
+    p
+  {{ fun ret => 0 ~> ret * 1 ~>? nat }} // StringMap.empty _).
+Proof.
+  (* This is a simple example which already seems much slower than necessary *)
+  Time compile. (* 4.2 seconds *)
+Defined.
+Eval lazy in (projT1 append_list_in_pair).
+
+Example match_option : sigT (fun p => forall env (o : option W) (r0 : W),
+  EXTRACT match o with
+  | Some t => Ret (S t)
+  | None => Ret 0
+  end
+  {{ 0 ~> o * 1 ~> r0 }}
+    p
+  {{ fun ret => 1 ~> ret * 0 |->? }} // env
+  ).
+Proof.
+  compile.
+Defined.
+
+Example find_in_map : sigT (fun p => forall env (m : Map.t W) (f0 : W),
+  EXTRACT (match Map.find (S f0) m with
+    | Some t => Ret (S t)
+    | None => Ret 0
+    end)
+  {{ 0 ~> m * 1 ~> f0}}
+    p
+  {{ fun ret => 0 |->? * 1 ~> ret }} // env).
+Proof.
+  intros. compile.
+Defined.
+
+Eval lazy in (projT1 find_in_map).
+
+Example add_to_map : sigT (fun p => forall env m,
+  EXTRACT (Ret (Map.add 1 5 m))
+  {{ 0 ~> m }}
+    p
+  {{ fun ret => 0 ~> ret }} // env).
+Proof.
+  intros. compile.
+Defined.
+
+Example remove_from_map : sigT (fun p => forall env (m : Map.t W),
+  EXTRACT (Ret (Map.remove 1 m))
+  {{ 0 ~> m }}
+    p
+  {{ fun ret => 0 ~> ret }} // env).
+Proof.
+  intros. compile.
+Defined.
+
+(*
+Instance prog_equiv_equivalence T :
+  Equivalence (@prog_equiv T).
+Proof.
+  split; hnf; unfold prog_equiv; firstorder.
+  eapply H0. eapply H. trivial.
+  eapply H. eapply H0. trivial.
+Qed.
+*)
+
+Example micro_add_twice : sigT (fun p => forall x,
+  EXTRACT Ret (1 + (2 + x))
+  {{ 0 ~> x }}
+    p
+  {{ fun ret => 0 ~> ret }} // StringMap.empty _).
+Proof.
+  compile.
+Defined.
+Eval lazy in projT1 micro_add_twice.
+
+Example micro_add_use_twice : sigT (fun p => forall x,
+  EXTRACT Ret (x + (2 + x))
+  {{ 0 ~> x }}
+    p
+  {{ fun ret => 0 ~> ret }} // StringMap.empty _).
+Proof.
+  compile.
+Defined.
+Eval lazy in projT1 micro_add_use_twice.
+
+Example compile_one_read : sigT (fun p =>
+  EXTRACT Read 1
+  {{ 0 ~> $0 }}
+    p
+  {{ fun ret => 0 ~> ret }} // StringMap.empty _).
+Proof.
+  compile.
+Defined.
+Eval lazy in projT1 (compile_one_read).
+
+Definition swap_prog a b :=
+  va <- Read a;
+  vb <- Read b;
+  Write a vb;;
+  Write b va;;
+  Ret tt.
+
+Example extract_swap_1_2 : forall env, sigT (fun p =>
+  EXTRACT swap_prog 1 2 {{ emp }} p {{ fun _ => emp }} // env).
+Proof.
+  intros. unfold swap_prog.
+  compile.
+Defined.
+Eval lazy in projT1 (extract_swap_1_2 (StringMap.empty _)).
+
+Lemma extract_swap_prog : forall env, sigT (fun p =>
+  forall a b F, EXTRACT swap_prog a b
+  {{ 0 ~> a * 1 ~> b * F }} p {{ fun _ => 0 |->? * 1 |->? * F}} // env).
+Proof.
+  intros. unfold swap_prog.
+  compile.
+Defined.
+Eval lazy in projT1 (extract_swap_prog (StringMap.empty _)).
+
+Example extract_increment : forall env, sigT (fun p => forall i,
+  EXTRACT (Ret (S i)) {{ 0 ~> i }} p {{ fun ret => 0 ~> ret }} // env).
+Proof.
+  intros.
+  compile.
+Defined.
+Eval lazy in projT1 (extract_increment (StringMap.empty _)).
+
+Example extract_for_loop : forall env, sigT (fun p =>
+  forall cnt nocrash crashed,
+  EXTRACT (@ForN_ W W (fun i sum => Ret (sum + i)) 1 cnt nocrash crashed 0)
+  {{ 0 ~> 0 * 1 ~> cnt }} p {{ fun ret => 0 ~> ret * 1 |->? }} // env).
+Proof.
+  intros.
+  compile.
+Defined.
+Eval lazy in projT1 (extract_for_loop (StringMap.empty _)).
+
+(*
+Declare DiskBlock
+  (fun var0 : nat =>
+   (DiskRead var0 (Var 0);
+    Declare DiskBlock
+      (fun var1 : nat =>
+       (DiskRead var1 (Var 1);
+        DiskWrite (Var 0) (Var var1);
+        DiskWrite (Var 1) (Var var0);
+        __)))%go)
+*)
+
+Opaque swap_prog.
+
+Definition extract_swap_prog_corr env := projT2 (extract_swap_prog env).
+Hint Resolve extract_swap_prog_corr : extractions.
+
+
+Definition swap_env : Env :=
+  ("swap" -s> {|
+           ParamVars := [(Go.Num, 0); (Go.Num, 1)];
+           RetParamVars := []; Body := projT1 (extract_swap_prog (StringMap.empty _));
+           (* ret_not_in_args := ltac:(auto); *) args_no_dup := ltac:(auto); body_source := ltac:(repeat constructor);
+         |}; (StringMap.empty _)).
+
+Lemma swap_func : voidfunc2 "swap" swap_prog swap_env.
+Proof.
+  unfold voidfunc2.
+  intros.
+  eapply extract_voidfunc2_call; eauto with extractions.
+  unfold swap_env; repeat rewrite ?StringMapFacts.add_eq_o, ?StringMapFacts.add_neq_o by congruence; reflexivity.
+Qed.
+Hint Resolve swap_func : funcs.
+
+Definition call_swap :=
+  swap_prog 0 1;;
+  Ret tt.
+
+Example extract_call_swap :
+  forall env,
+    voidfunc2 "swap" swap_prog env ->
+    sigT (fun p =>
+          EXTRACT call_swap {{ emp }} p {{ fun _ => emp }} // env).
+Proof.
+  unfold call_swap.
+  intros.
+  compile.
+Defined.
+
+Example extract_call_swap_top :
+    sigT (fun p =>
+          EXTRACT call_swap {{ emp }} p {{ fun _ => emp }} // swap_env).
+Proof.
+  apply extract_call_swap.
+  auto with funcs.
+Defined.
+Eval lazy in projT1 (extract_call_swap_top).
+
+Definition rot3_prog :=
+  swap_prog 0 1;;
+  swap_prog 1 2;;
+  Ret tt.
+
+Example extract_rot3_prog :
+  forall env,
+    voidfunc2 "swap" swap_prog env ->
+    sigT (fun p =>
+          EXTRACT rot3_prog {{ emp }} p {{ fun _ => emp }} // env).
+Proof.
+  intros.
+  unfold rot3_prog.
+  repeat (compile_step; try solve [unfold exis' at 3; cancel]). (* TODO something with cancel_go *)
+  Unshelve. compile.
+Defined.
+
+Example extract_rot3_prog_top :
+    sigT (fun p =>
+          EXTRACT rot3_prog {{ emp }} p {{ fun _ => emp }} // swap_env).
+Proof.
+  apply extract_rot3_prog.
+  auto with funcs.
+Defined.
+Eval lazy in projT1 (extract_rot3_prog_top).
+(*
+(Declare Num
+   (fun var0 : W =>
+    (var0 <~ Const Num 1;
+     Declare Num
+       (fun var1 : W =>
+        (var1 <~ Const Num 0;
+         Call [] "swap" [var1; var0]))));
+ Declare Num
+   (fun var0 : W =>
+    (var0 <~ Const Num 2;
+     Declare Num
+       (fun var1 : W =>
+        (var1 <~ Const Num 1;
+         Call [] "swap" [var1; var0]))));
+ __)%go
+*)
+
+
+Definition swap2_prog :=
+  a <- Read 0;
+  b <- Read 1;
+  if weq a b then
+    Ret tt
+  else
+    Write 0 b;;
+    Write 1 a;;
+    Ret tt.
+
+(*
+Example micro_swap2 : sigT (fun p =>
+  EXTRACT swap2_prog {{ emp }} p {{ fun _ => emp }} // (StringMap.empty _)).
+Proof.
+  compile.
+
+  eapply hoare_weaken_post; [ | eapply CompileIf with (condvar := "c0") (retvar := "r") ];
+    try match_scopes; maps.
+
+  apply GoWrapper_unit.
+  compile. apply H.
+
+  compile.
+  eapply CompileWeq.
+
+  shelve.
+  shelve.
+  shelve.
+
+  eapply hoare_strengthen_pre.
+  2: eapply CompileVar.
+  match_scopes.
+
+  intros.
+  eapply hoare_strengthen_pre.
+  2: eapply CompileVar.
+  match_scopes.
+
+  Unshelve.
+  all: congruence.
+Defined.
+Eval lazy in projT1 micro_swap2.
+*)
 
 Example swap_example : stmt :=
   (Declare Num (fun a =>
