src/GoCompilationLemmas.v
@@ -1,0 +1,1568 @@
+Require Import Eqdep.
+Require Import PeanoNat Plus List.
+Require Import Word AsyncDisk Prog ProgMonad BasicProg Pred SepAuto.
+Require Import StringMap.
+Require Import GoSemantics GoFacts GoHoare.
+Require Import GoTactics2.
+
+Import ListNotations.
+
+Set Implicit Arguments.
+
+
+Hint Constructors step fail_step crash_step exec.
+
+Hint Extern 1 (Go.eval _ _ = _) =>
+unfold Go.eval.
+
+Hint Extern 1 (Go.step _ (_, Go.Assign _ _) _) =>
+  eapply Go.StepAssign.
+Hint Constructors Go.step.
+
+
+
+Lemma CompileSkip : forall env A,
+  EXTRACT Ret tt
+  {{ A }}
+    Go.Skip
+  {{ fun _ => A }} // env.
+Proof.
+  unfold ProgOk.
+  intros.
+  inv_exec_progok.
+Qed.
+
+
+Lemma CompileConst : forall env A var (v : nat),
+  EXTRACT Ret v
+  {{ var ~>? W * A }}
+    var <~const v
+  {{ fun ret => var ~> ret * A }} // env.
+Proof.
+  unfold ProgOk.
+  intros.
+  inv_exec_progok.
+  eval_expr.
+  do 2 eexists.
+  intuition eauto.
+  pred_solve.
+
+  eval_expr.
+  contradiction H1.
+  repeat econstructor; eauto.
+  eval_expr.
+  reflexivity.
+Qed.
+
+Lemma CompileRet : forall T {H: GoWrapper T} env A B var (v : T) p,
+  EXTRACT Ret v
+  {{ A }}
+    p
+  {{ fun ret => var ~> ret * B }} // env ->
+  EXTRACT Ret tt
+  {{ A }}
+    p
+  {{ fun _ => var ~> v * B }} // env.
+Proof.
+  unfold ProgOk; intros.
+  forward_solve.
+  - invc H4;
+    repeat find_apply_lem_hyp inj_pair2; repeat subst;
+    eauto.
+    invc H14.
+  - invc H0.
+    repeat find_apply_lem_hyp inj_pair2; repeat subst.
+    invc H10.
+  - invc H5.
+    repeat find_apply_lem_hyp inj_pair2; repeat subst.
+    invc H10.
+
+  Unshelve.
+  all: auto.
+Qed.
+
+Lemma CompileRet' : forall T {H: GoWrapper T} env A B var (v : T) p,
+  EXTRACT Ret tt
+  {{ A }}
+    p
+  {{ fun _ => var ~> v * B }} // env ->
+  EXTRACT Ret v
+  {{ A }}
+    p
+  {{ fun ret => var ~> ret * B }} // env.
+Proof.
+  unfold ProgOk; intros.
+  forward_solve.
+  - invc H4;
+    repeat find_apply_lem_hyp inj_pair2; repeat subst;
+    eauto.
+    invc H14.
+  - invc H0.
+    repeat find_apply_lem_hyp inj_pair2; repeat subst.
+    invc H10.
+  - invc H5.
+    repeat find_apply_lem_hyp inj_pair2; repeat subst.
+    invc H10.
+
+  Unshelve.
+  all: auto.
+Qed.
+
+Lemma CompileConst' : forall env A var (v : nat),
+  EXTRACT Ret tt
+  {{ var ~>? nat * A }}
+    var <~const v
+  {{ fun _ => var ~> v * A }} // env.
+Proof.
+  eauto using CompileRet, CompileConst.
+Qed.
+
+Import Go.
+
+Inductive Declaration :=
+| Decl (T : Type) {Wr: GoWrapper T} {D : DefaultValue T}.
+
+Arguments Decl T {Wr} {D}.
+
+Fixpoint n_tuple_unit n (T : Type) : Type :=
+  match n with
+  | 0 => unit
+  | S n' => n_tuple_unit n' T * T
+  end.
+
+Definition decls_pre (decls : list Declaration) (vars : n_tuple_unit (length decls) var) : pred.
+  induction decls; simpl in *.
+  - exact emp.
+  - destruct a.
+    exact ((snd vars |-> wrap zeroval * IHdecls (fst vars))%pred).
+Defined.
+
+Definition decls_post (decls : list Declaration) (vars : n_tuple_unit (length decls) var) : pred.
+  induction decls; simpl in *.
+  - exact emp.
+  - exact ((snd vars |->? * IHdecls (fst vars))%pred).
+Defined.
+
+Lemma decls_pre_impl_post :
+  forall decls vars,
+    decls_pre decls vars =p=> decls_post decls vars.
+Proof.
+  induction decls; simpl in *; intros.
+  - auto.
+  - destruct a.
+    cancel. auto.
+Qed.
+Hint Resolve decls_pre_impl_post : cancel_go_finish.
+
+Local Open Scope map_scope.
+
+Lemma Declare_fail :
+  forall env d s t xp,
+    Go.exec env (d, s, Go.Declare t xp) Go.Failed ->
+    exists var, Go.exec env (d, var ->> Go.default_value t; s,
+      (xp var; Go.Undeclare var)%go) Go.Failed /\ VarMap.find var s = None.
+Proof.
+  intros.
+  invc H.
+  + invc H0; eauto.
+  + exfalso; eauto using can_always_declare.
+Qed.
+
+Lemma Undeclare_fail :
+  forall env st var,
+    Go.exec env (st, Go.Undeclare var) Go.Failed -> False.
+Proof.
+  intros.
+  invc H.
+  + repeat inv_exec; auto.
+  + contradiction H0. destruct st. repeat econstructor.
+Qed.
+
+Lemma CompileDeclare :
+  forall env R T {Wr : GoWrapper T} {WrD : DefaultValue T} A B (p : prog R) xp,
+    (forall var,
+       EXTRACT p
+       {{ var ~> zeroval * A }}
+         xp var
+       {{ fun ret => var |->? * B ret }} // env) ->
+    EXTRACT p
+    {{ A }}
+      Go.Declare wrap_type xp
+    {{ fun ret => B ret }} // env.
+Proof.
+  unfold ProgOk; intros.
+  repeat destruct_pair.
+  destruct out; intuition try discriminate; simpl in *.
+  - find_apply_lem_hyp Declare_fail; repeat deex.
+
+    specialize (H x (r, x ->> Go.default_value wrap_type; l) hm).
+    forward H.
+    {
+      simpl. pred_solve.
+    }
+    intuition idtac.
+    find_apply_lem_hyp Go.ExecFailed_Steps.
+    forward_solve.
+    find_apply_lem_hyp Go.Steps_Seq.
+    forward_solve.
+
+    + find_apply_lem_hyp Go.Steps_ExecFailed; eauto.
+      forward_solve.
+      cbv [snd Go.is_final]. intuition (subst; eauto).
+      forward_solve.
+
+    + exfalso; eauto using Undeclare_fail, Go.Steps_ExecFailed.
+
+  - do 2 inv_exec.
+    specialize (H var0 (r, var0 ->> Go.default_value wrap_type; l) hm).
+    forward H.
+    {
+      simpl. pred_solve.
+    }
+    destruct_pair.
+    find_inversion_safe.
+    find_eapply_lem_hyp Go.ExecFinished_Steps.
+    find_eapply_lem_hyp Go.Steps_Seq.
+    forward_solve.
+    repeat find_eapply_lem_hyp Go.Steps_ExecFinished.
+    invc H4. invc H. invc H5. invc H.
+    forward_solve.
+    simpl in *.
+    repeat eexists; eauto.
+    pred_solve.
+
+  - do 2 inv_exec.
+    specialize (H var0 (r, var0 ->> Go.default_value wrap_type; l) hm).
+    forward H.
+    {
+      simpl. pred_solve.
+    }
+    find_inversion_safe.
+    find_eapply_lem_hyp Go.ExecCrashed_Steps.
+    repeat deex; try discriminate.
+    find_eapply_lem_hyp Go.Steps_Seq.
+    intuition idtac.
+    + repeat deex.
+      invc H4.
+      eapply Go.Steps_ExecCrashed in H2; eauto.
+      simpl in *.
+      forward_solve.
+    + deex.
+      invc H5; [ invc H4 | invc H ].
+      invc H6; [ invc H4 | invc H ].
+Qed.
+
+Definition many_declares (decls : list Declaration) (xp : n_tuple_unit (length decls) var -> stmt) : stmt.
+  induction decls; simpl in *.
+  - exact (xp tt).
+  - destruct a.
+    eapply (Declare wrap_type); intro var.
+    apply IHdecls; intro.
+    apply xp.
+    exact (X, var).
+Defined.
+
+Lemma CompileDeclareMany :
+  forall env T (decls : list Declaration) xp A B (p : prog T),
+    (forall vars : n_tuple_unit (length decls) var,
+       EXTRACT p
+       {{ decls_pre decls vars * A }}
+         xp vars
+       {{ fun ret => decls_post decls vars * B ret }} // env) ->
+    EXTRACT p
+    {{ A }}
+      many_declares decls xp
+    {{ fun ret => B ret }} // env.
+Proof.
+  induction decls; simpl; intros.
+  - eapply hoare_weaken; [ apply H | cancel_go.. ].
+  - destruct a. eapply CompileDeclare; eauto. intros.
+    eapply IHdecls. intros.
+    eapply hoare_weaken; [ apply H | cancel_go.. ].
+Qed.
+
+Lemma CompileVar : forall env A var T (v : T) {H : GoWrapper T},
+  EXTRACT Ret v
+  {{ var ~> v * A }}
+    Go.Skip
+  {{ fun ret => var ~> ret * A }} // env.
+Proof.
+  unfold ProgOk.
+  intros.
+  inv_exec_progok.
+Qed.
+
+Lemma CompileBind : forall T T' {H: GoWrapper T} env A B (C : T' -> _) v0 p f xp xf var,
+  EXTRACT p
+  {{ var ~> v0 * A }}
+    xp
+  {{ fun ret => var ~> ret * B }} // env ->
+  (forall (a : T),
+    EXTRACT f a
+    {{ var ~> a * B }}
+      xf
+    {{ C }} // env) ->
+  EXTRACT Bind p f
+  {{ var ~> v0 * A }}
+    xp; xf
+  {{ C }} // env.
+Proof.
+  unfold ProgOk.
+  intuition subst.
+
+  - find_eapply_lem_hyp Go.ExecFinished_Steps. find_eapply_lem_hyp Go.Steps_Seq.
+    intuition; repeat deex; try discriminate.
+    find_eapply_lem_hyp Go.Steps_ExecFinished. find_eapply_lem_hyp Go.Steps_ExecFinished.
+    forwardauto H0; intuition.
+    forwardauto H3; repeat deex.
+    specialize (H1 x0).
+    forward_solve.
+
+  - find_eapply_lem_hyp Go.ExecCrashed_Steps. repeat deex. find_eapply_lem_hyp Go.Steps_Seq.
+    intuition; repeat deex.
+    + invc H5. find_eapply_lem_hyp Go.Steps_ExecCrashed; eauto.
+      forward_solve.
+    + destruct x1. find_eapply_lem_hyp Go.Steps_ExecFinished. find_eapply_lem_hyp Go.Steps_ExecCrashed; eauto.
+      forwardauto H0; intuition.
+      forwardauto H3; repeat deex.
+      specialize (H1 x1).
+      forward_solve.
+
+  - find_eapply_lem_hyp Go.ExecFailed_Steps. repeat deex. find_eapply_lem_hyp Go.Steps_Seq.
+    intuition; repeat deex.
+    + eapply Go.Steps_ExecFailed in H5; eauto.
+      forward_solve.
+      unfold Go.is_final; simpl; intuition subst.
+      contradiction H6. eauto.
+      intuition. repeat deex.
+      contradiction H6. eauto.
+    + destruct x1. find_eapply_lem_hyp Go.Steps_ExecFinished. find_eapply_lem_hyp Go.Steps_ExecFailed; eauto.
+      forwardauto H0; intuition.
+      forwardauto H4; repeat deex.
+      specialize (H1 x1).
+      forward_solve.
+Qed.
+
+
+Lemma CompileSeq : forall T T' env A B (C : T -> _) p1 p2 x1 x2,
+  EXTRACT p1
+  {{ A }}
+    x1
+  {{ fun _ => B }} // env ->
+  EXTRACT p2
+  {{ B }}
+    x2
+  {{ C }} // env ->
+  EXTRACT Bind p1 (fun _ : T' => p2)
+  {{ A }}
+    x1; x2
+  {{ C }} // env.
+Proof.
+  unfold ProgOk.
+  intuition subst.
+
+  - find_eapply_lem_hyp ExecFinished_Steps. find_eapply_lem_hyp Steps_Seq.
+    intuition; repeat deex; try discriminate.
+    find_eapply_lem_hyp Steps_ExecFinished. find_eapply_lem_hyp Steps_ExecFinished.
+    (* [forward_solve] is not really good enough *)
+    forwardauto H. intuition.
+    forwardauto H2. repeat deex.
+    forward_solve.
+
+  - find_eapply_lem_hyp ExecCrashed_Steps. repeat deex. find_eapply_lem_hyp Steps_Seq.
+    intuition; repeat deex.
+    + invc H4. find_eapply_lem_hyp Steps_ExecCrashed; eauto.
+      forward_solve.
+    + destruct x3. find_eapply_lem_hyp Steps_ExecFinished. find_eapply_lem_hyp Steps_ExecCrashed; eauto.
+      forwardauto H. intuition.
+      forwardauto H2. repeat deex.
+      forward_solve.
+
+  - find_eapply_lem_hyp ExecFailed_Steps. repeat deex. find_eapply_lem_hyp Steps_Seq.
+    intuition; repeat deex.
+    + eapply Steps_ExecFailed in H4; eauto.
+      forward_solve.
+      unfold is_final; simpl; intuition subst.
+      contradiction H5.
+      repeat eexists. eauto.
+      intuition. repeat deex.
+      contradiction H5. eauto.
+    + destruct x3. find_eapply_lem_hyp Steps_ExecFinished. find_eapply_lem_hyp Steps_ExecFailed; eauto.
+      forwardauto H. intuition.
+      forwardauto H3. repeat deex.
+      forward_solve.
+
+  Unshelve.
+  all: auto.
+Qed.
+
+Lemma CompileBindDiscard : forall T T' env A (B : T' -> _)
+  (p : prog T) (f : prog T') xp xf,
+  EXTRACT p
+  {{ A }}
+    xp
+  {{ fun _ => A }} // env ->
+  EXTRACT f
+  {{ A }}
+    xf
+  {{ B }} // env ->
+  EXTRACT Bind p (fun (_ : T) => f)
+  {{ A }}
+    xp; xf
+  {{ B }} // env.
+Proof.
+  intros.
+  eapply CompileSeq; eauto.
+Qed.
+
+Lemma CompileBefore : forall T env A B (C : T -> _) p x1 x2,
+  EXTRACT Ret tt
+  {{ A }}
+    x1
+  {{ fun _ => B }} // env ->
+  EXTRACT p
+  {{ B }}
+    x2
+  {{ C }} // env ->
+  EXTRACT p
+  {{ A }}
+    x1; x2
+  {{ C }} // env.
+Proof.
+  intros.
+  eapply extract_equiv_prog with (pr1 := Ret tt;; p).
+  eapply bind_left_id.
+  eapply CompileSeq; eauto.
+Qed.
+
+Lemma CompileAfter : forall T env A B (C : T -> _) p x1 x2,
+  EXTRACT p
+  {{ A }}
+    x1
+  {{ B }} // env ->
+  (forall r : T,
+      EXTRACT Ret tt
+      {{ B r }}
+        x2
+      {{ fun _ => C r }} // env) ->
+  EXTRACT p
+  {{ A }}
+    x1; x2
+  {{ C }} // env.
+Proof.
+  unfold ProgOk.
+  intuition subst.
+
+  - find_eapply_lem_hyp ExecFinished_Steps. find_eapply_lem_hyp Steps_Seq.
+    intuition; repeat deex; try discriminate.
+    find_eapply_lem_hyp Steps_ExecFinished. find_eapply_lem_hyp Steps_ExecFinished.
+    (* [forward_solve] is not really good enough *)
+    forwardauto H. intuition.
+    forwardauto H2. repeat deex.
+    forward_solve.
+    invc H8; repeat (find_apply_lem_hyp inj_pair2; subst); [ | invc H18 ]; eauto.
+
+  - find_eapply_lem_hyp ExecCrashed_Steps. repeat deex. find_eapply_lem_hyp Steps_Seq.
+    intuition; repeat deex.
+    + invc H4. find_eapply_lem_hyp Steps_ExecCrashed; eauto.
+      forward_solve.
+    + destruct x3. find_eapply_lem_hyp Steps_ExecFinished. find_eapply_lem_hyp Steps_ExecCrashed; eauto.
+      forwardauto H. intuition.
+      forwardauto H2. repeat deex.
+      forward_solve.
+      invc H0.
+      repeat (find_apply_lem_hyp inj_pair2; subst).
+      invc H15.
+
+  - find_eapply_lem_hyp ExecFailed_Steps. repeat deex. find_eapply_lem_hyp Steps_Seq.
+    intuition; repeat deex.
+    + eapply Steps_ExecFailed in H4; eauto.
+      forward_solve.
+      unfold is_final; simpl; intuition subst.
+      contradiction H5.
+      repeat eexists. eauto.
+      intuition. repeat deex.
+      contradiction H5. eauto.
+    + destruct x3. find_eapply_lem_hyp Steps_ExecFinished. find_eapply_lem_hyp Steps_ExecFailed; eauto.
+      forwardauto H. intuition.
+      forwardauto H3. repeat deex.
+      forward_solve.
+      invc H10.
+      repeat (find_apply_lem_hyp inj_pair2; subst).
+      invc H15.
+
+  Unshelve.
+  all: auto.
+Qed.
+
+Lemma CompileBindRet : forall A B (HA : GoWrapper A)
+  vara (a : A) (p : A -> prog B) xp xret X Y Z env,
+  EXTRACT (Ret a)
+  {{ vara ~>? A * X }}
+    xret
+  {{ fun ret => vara ~> ret * Y }} // env ->
+  EXTRACT (p a)
+  {{ vara ~> a * Y }}
+    xp
+  {{ Z }} // env ->
+  EXTRACT (Bind (Ret a) p)
+  {{ vara ~>? A * X }}
+    xret; xp
+  {{ Z }} // env.
+Proof.
+  intros.
+  eapply CompileBefore in H0.
+  rewrite bind_left_id.
+  eapply H0.
+  eapply CompileRet. eapply H.
+Qed.
+
+Lemma CompileWeq : forall A (a b : valu) env xa xb retvar avar bvar,
+  EXTRACT Ret a
+  {{ A }}
+    xa
+  {{ fun ret => avar ~> ret * A }} // env ->
+  (forall (av : valu),
+  EXTRACT Ret b
+  {{ avar ~> av * A }}
+    xb
+  {{ fun ret => bvar ~> ret * avar ~> av * A }} // env) ->
+  EXTRACT Ret (weq a b)
+  {{ A }}
+    xa ; xb ; retvar <~ (Var avar = Var bvar)
+  {{ fun ret => retvar ~> ret * A }} // env.
+Proof.
+  unfold ProgOk.
+  intuition.
+Admitted.
+
+Lemma CompileIf : forall V varb (b : bool)
+  (ptrue pfalse : prog V) xptrue xpfalse F G env,
+  EXTRACT ptrue
+  {{ varb ~> true * F }}
+    xptrue
+  {{ fun ret => G ret * varb ~>? bool }} // env ->
+  EXTRACT pfalse
+  {{ varb ~> false * F }}
+    xpfalse
+  {{ fun ret => G ret * varb ~>? bool }} // env ->
+  EXTRACT (if b then ptrue else pfalse)
+  {{ varb ~> b * F }}
+    If (Var varb) Then xptrue Else xpfalse EndIf
+  {{ fun ret => G ret * varb ~>? bool }} // env.
+Proof.
+  intros. unfold ProgOk.
+  inv_exec_progok.
+  all : inv_exec; try inv_exec; eval_expr;
+    try match goal with
+    [ H : context [ProgOk] |- _] =>
+      solve [edestruct H; forward_solve; pred_solve]
+    end.
+  all : contradiction H3;
+    repeat eexists; solve [
+    eapply StepIfTrue; eval_expr |
+    eapply StepIfFalse; eval_expr].
+Qed.
+
+Lemma CompileRead :
+  forall env F avar vvar (v0 : valu) a,
+    EXTRACT Read a
+    {{ vvar ~> v0 * avar ~> a * F }}
+      DiskRead vvar (Var avar)
+    {{ fun ret => vvar ~> ret * avar ~> a * F }} // env.
+Proof.
+  unfold ProgOk.
+  intros.
+  inv_exec_progok.
+  {
+    eval_expr.
+    repeat eexists; eauto.
+    pred_solve.
+  }
+  destruct (r a) as [p|] eqn:H'; eauto.
+  destruct p.
+  contradiction H1.
+  repeat econstructor; eauto.
+  all : eval_expr; eauto.
+Qed.
+
+Lemma CompileWrite : forall env F avar vvar a v,
+  EXTRACT Write a v
+  {{ avar ~> a * vvar ~> v * F }}
+    DiskWrite (Var avar) (Var vvar)
+  {{ fun _ => avar ~> a * vvar ~> v * F }} // env.
+Proof.
+  unfold ProgOk.
+  intros.
+  inv_exec_progok.
+  {
+    eval_expr.
+    repeat eexists; eauto.
+  }
+  destruct (r a) as [p|] eqn:H'; eauto.
+  destruct p.
+  contradiction H1.
+  repeat eexists; eauto.
+  econstructor; eauto.
+  all : eval_expr; eauto.
+Qed.
+
+
+Lemma CompileAdd :
+  forall env F sumvar avar bvar (a b : nat),
+    EXTRACT Ret (a + b)
+    {{ sumvar ~>? W * avar ~> a * bvar ~> b * F }}
+      Modify (ModifyNumOp Plus) (sumvar, avar, bvar)
+    {{ fun ret => sumvar ~> ret * avar ~> a * bvar ~> b * F }} // env.
+Proof.
+  unfold ProgOk; intros.
+  destruct_pair; simpl in *.
+  inv_exec_progok.
+  eval_expr.
+  repeat econstructor.
+  pred_solve.
+
+  contradiction H1.
+  eval_expr.
+  repeat econstructor.
+  all: eval_expr; [reflexivity].
+Qed.
+
+Lemma CompileAddInPlace1 :
+  forall env F avar bvar (a b : nat),
+    EXTRACT Ret (a + b)
+    {{ avar ~> a * bvar ~> b * F }}
+      Modify (ModifyNumOp Plus) (avar, avar, bvar)
+    {{ fun ret => avar ~> ret * bvar ~> b * F }} // env.
+Proof.
+  unfold ProgOk; intros.
+  destruct_pair; simpl in *.
+  inv_exec_progok.
+  eval_expr.
+  repeat econstructor.
+  pred_solve.
+
+  contradiction H1.
+  eval_expr.
+  repeat econstructor.
+  all: eval_expr; [reflexivity].
+Qed.
+
+(* TODO: make it unnecessary to have all these separate lemmas *)
+Lemma CompileAddInPlace2 :
+  forall env F avar bvar (a b : nat),
+    EXTRACT Ret (a + b)
+    {{ avar ~> a * bvar ~> b * F }}
+      Modify (ModifyNumOp Plus) (bvar, avar, bvar)
+    {{ fun ret => bvar ~> ret * avar ~> a * F }} // env.
+Proof.
+  unfold ProgOk; intros.
+  destruct_pair; simpl in *.
+  inv_exec_progok.
+  eval_expr.
+  repeat econstructor.
+  pred_solve.
+
+  contradiction H1.
+  eval_expr.
+  repeat econstructor.
+  all: eval_expr; [reflexivity].
+Qed.
+
+Lemma CompileAppend :
+  forall env F T {Wr: GoWrapper T} (lvar vvar : var) (x : T) xs,
+  EXTRACT Ret (x :: xs)
+  {{ vvar ~> x * lvar ~> xs * F }}
+    Modify AppendOp (lvar, vvar)
+  {{ fun ret => vvar |-> moved_value (wrap x) * lvar ~> ret * F }} // env.
+Proof.
+  unfold ProgOk; intros.
+  repeat extract_var_val.
+  inv_exec_progok.
+  - find_apply_lem_hyp inj_pair2; subst.
+    simpl in *.
+    repeat find_rewrite.
+    unfold append_impl, append_impl', update_one, id in *.
+    repeat destruct_pair.
+    repeat find_inversion_safe.
+    simpl in *. subst.
+    rewrite ?eq_dec_eq in *.
+    repeat find_inversion_safe.
+    simpl in *.
+    rewrite ?eq_dec_eq in *.
+    repeat find_inversion_safe.
+    destruct (can_alias wrap_type); simpl in *.
+    + rewrite ?eq_dec_eq in *. simpl in *. find_inversion; simpl in *.
+      repeat eexists.
+      eauto.
+      pred_solve.
+    + rewrite ?eq_dec_eq in *; simpl in *.
+      find_inversion.
+      repeat econstructor.
+      pred_solve.
+
+  - contradiction H1.
+    repeat eexists; econstructor.
+    unfold append_impl'. simpl.
+    (* TODO: this is a mess *)
+    all: unfold sel; simpl; repeat find_rewrite; try reflexivity; repeat (simpl; rewrite eq_dec_eq in * ); try reflexivity.
+    simpl.
+    rewrite ?eq_dec_eq in *.
+    simpl.
+    instantiate (1 := ltac:(destruct (can_alias wrap_type))).
+    destruct (can_alias wrap_type); simpl in *.
+    + rewrite ?eq_dec_eq; reflexivity.
+    + reflexivity.
+Qed.
+
+
+
+Lemma map_add_okToUnify : forall AT AEQ {T} {Wr : GoWrapper T} var m k (v : T),
+  (@okToUnify AT AEQ value (var ~> Map.add k v m)
+  (var |-> (Val (AddrMap wrap_type) (Here (Map.add k (wrap' v) (Map.map wrap' m))))))%pred.
+Proof.
+  intros. unfold okToUnify.
+  unfold wrap. simpl. repeat f_equal.
+  eauto using MapUtils.addrmap_equal_eq,
+    MoreAddrMapFacts.map_add_comm,
+    MapUtils.AddrMap.MapFacts.Equal_refl.
+Qed.
+
+Hint Extern 1 (okToUnify (?var ~> Map.add ?k ?v ?m)
+  (?var |-> (Val (AddrMap wrap_type) (Here (Map.add ?k (wrap' ?v) (Map.map wrap' ?m))))))
+  => apply map_add_okToUnify.
+
+
+Lemma map_remove_okToUnify : forall AT AEQ {T} {Wr : GoWrapper T} var m k,
+  (@okToUnify AT AEQ value (var ~> Map.remove k m)
+  (var |-> (Val (AddrMap wrap_type) (Here (Map.remove k (Map.map wrap' m))))))%pred.
+Proof.
+  intros. unfold okToUnify.
+  unfold wrap. simpl. repeat f_equal.
+  eauto using MapUtils.addrmap_equal_eq,
+    MoreAddrMapFacts.map_remove_comm,
+    MapUtils.AddrMap.MapFacts.Equal_refl.
+Qed.
+
+Local Hint Extern 1 (okToUnify (?var ~> Map.remove ?k ?m)
+  (?var |-> (Val (AddrMap wrap_type) (Here (Map.remove ?k (Map.map wrap' ?m))))))
+  => apply map_remove_okToUnify.
+
+
+Lemma map_find_some_okToUnify : forall AT AEQ {T} {Wr : GoWrapper T} var m k v,
+  Map.find k (Map.map wrap' m) = Some v ->
+  (@okToUnify AT AEQ value (var ~> Map.find k m)
+  (var |-> Val (Pair Bool wrap_type) (true, v))).
+Proof.
+  intros. unfold okToUnify, wrap. simpl.
+  rewrite MapUtils.AddrMap.MapFacts.map_o in H.
+  destruct Map.find; simpl in *; congruence.
+Qed.
+
+Lemma map_find_none_okToUnify : forall AT AEQ {T} {Wr : GoWrapper T} var m k,
+  Map.find k (Map.map wrap' m) = None ->
+  (@okToUnify AT AEQ value (var ~> Map.find k m)
+  (var |-> Val (Pair Bool wrap_type) (false, default_value' wrap_type))).
+Proof.
+  intros. unfold okToUnify, wrap. simpl.
+  rewrite MapUtils.AddrMap.MapFacts.map_o in H.
+  destruct Map.find; simpl in *; congruence.
+Qed.
+
+Local Hint Extern 1 (okToUnify (?var ~> Map.find ?k ?m)
+  (?var |-> (Val (Pair Bool wrap_type) (true, ?v))))
+  => eapply map_find_some_okToUnify.
+
+Local Hint Extern 1 (okToUnify (?var ~> Map.find ?k ?m)
+  (?var |-> (Val (Pair Bool wrap_type) (false, ?v))))
+  => eapply map_find_none_okToUnify.
+
+
+Lemma CompileMapAdd : forall env F T {Wr : GoWrapper T} mvar kvar vvar m k (v : T),
+  EXTRACT Ret (Go.Map.add k v m)
+  {{ mvar ~> m * kvar ~> k * vvar ~> v * F }}
+    Go.Modify Go.MapAdd (mvar, kvar, vvar)
+  {{ fun ret => mvar ~> ret * kvar ~> k * vvar |-> moved_value (wrap v) * F }} // env.
+Proof.
+  unfold ProgOk.
+  repeat inv_exec_progok.
+  - eval_expr; [ repeat eexists; eauto; pred_solve..].
+  - eval_expr.
+    repeat (contradiction H1;
+    repeat econstructor; eauto;
+    [ eval_expr; eauto ..]).
+Qed.
+
+
+Lemma CompileMapRemove : forall env F T {Wr : GoWrapper T} mvar kvar m k,
+  EXTRACT Ret (Go.Map.remove k m)
+  {{ mvar ~> m * kvar ~> k * F }}
+    Go.Modify Go.MapRemove (mvar, kvar)
+  {{ fun ret => mvar ~> ret * kvar ~> k * F }} // env.
+Proof.
+  unfold ProgOk.
+  repeat inv_exec_progok.
+  - eval_expr; [ repeat eexists; eauto; pred_solve..].
+  - eval_expr.
+    repeat (contradiction H1;
+    repeat econstructor; eauto;
+    [ eval_expr; eauto ..]).
+Qed.
+
+Lemma CompileMapFind : forall env F T {Wr : GoWrapper T} mvar kvar vvar m k,
+  EXTRACT Ret (Go.Map.find k m)
+  {{ mvar ~> m * kvar ~> k * vvar ~>? (option T) * F }}
+    Go.Modify Go.MapFind (mvar, kvar, vvar)
+  {{ fun ret => vvar ~> ret * mvar ~> m * kvar ~> k * F }} // env.
+Proof.
+  unfold ProgOk.
+  repeat inv_exec_progok.
+  - eval_expr.
+    repeat eexists; eauto. pred_solve.
+    repeat eexists; eauto. pred_solve.
+  - eval_expr.
+    repeat (contradiction H1;
+    repeat econstructor;
+    [ eval_expr; eauto..]).
+Qed.
+
+Lemma map_cardinal_okToUnify : forall AT AEQ {T} {Wr : GoWrapper T} var m,
+  (@okToUnify AT AEQ value (var ~> Map.cardinal m)
+  (var |-> (Val Num (Here (Map.cardinal (Map.map wrap' m))))))%pred.
+Proof.
+  intros. unfold okToUnify.
+  unfold wrap. simpl. repeat f_equal. unfold id.
+  eauto using MapUtils.AddrMap.map_cardinal_map_eq.
+Qed.
+
+Local Hint Extern 1 (okToUnify (?var ~> Map.cardinal ?m)
+  (?var |-> (Val Num (Here (Map.cardinal (Map.map wrap' ?m))))))
+  => apply map_cardinal_okToUnify.
+
+Lemma CompileMapCardinal : forall env F T {Wr : GoWrapper T} mvar m var (v0 : W),
+  EXTRACT Ret (Go.Map.cardinal m)
+  {{ var ~> v0 * mvar ~> m * F }}
+    Go.Modify Go.MapCardinality (mvar, var)
+  {{ fun ret => var ~> ret * mvar ~> m * F }} // env.
+Proof.
+  unfold ProgOk.
+  repeat inv_exec_progok.
+  - eval_expr.
+    repeat eexists; eauto. pred_solve.
+  - contradiction H1.
+    repeat econstructor; [ eval_expr; eauto..].
+Qed.
+
+Lemma map_elements_okToUnify : forall AT AEQ {T} {Wr : GoWrapper T} var m,
+  @okToUnify AT AEQ value (var ~> Map.elements m)
+  (var |-> Val (Slice (Pair Num wrap_type))
+         (Here (map (fun x => (Here (fst x), snd x))
+               (Map.elements (Map.map wrap' m))))).
+Proof.
+  intros.
+  unfold okToUnify.
+  unfold wrap; simpl wrap. repeat f_equal.
+  simpl wrap'. repeat f_equal.
+  rewrite MapUtils.AddrMap.map_elements_map_eq.
+  rewrite map_map. simpl. reflexivity.
+Qed.
+
+Local Hint Extern 1 (okToUnify (?var ~> Map.elements ?k ?m)
+  (?var |-> (Val _ (Here (map _ (Map.elements _))))))
+  => eapply map_elements_okToUnify : okToUnify.
+
+Local Hint Extern 1 (okToUnify (?var ~> Map.elements _)
+  (?var |-> Val _ (Here(map _
+   (MapUtils.AddrMap_List.Raw.map wrap' (MapUtils.AddrMap_List.this _))))))
+  => eapply map_elements_okToUnify : okToUnify.
+
+Lemma CompileMapElements : forall env F T {Wr : GoWrapper T} mvar m var (v0 : list (W * T)),
+  EXTRACT Ret (Go.Map.elements m)
+  {{ var ~> v0 * mvar ~> m * F }}
+    Go.Modify Go.MapElements (mvar, var)
+  {{ fun ret => var ~> ret * mvar ~> m * F }} // env.
+Proof.
+  unfold ProgOk.
+  repeat inv_exec_progok.
+  - eval_expr.
+    repeat eexists; eauto. pred_solve.
+  - eval_expr.
+    contradiction H1. repeat econstructor.
+    eval_expr. eauto.
+    eval_expr. eauto.
+    eval_expr. eauto.
+Qed.
+
+Lemma CompileForLoopBasic : forall L G (L' : GoWrapper L) v loopvar F
+                          (n i : W)
+                          t0 term
+                          env (pb : W -> L -> prog L) xpb nocrash oncrash,
+    (forall t x,
+        EXTRACT (pb x t)
+  {{ loopvar ~> t * v ~> x * term ~> (i + n) * F }}
+    xpb
+  {{ fun ret => loopvar ~> ret * v ~> S x * term ~> (i + n) * F }} // env)
+  ->
+  EXTRACT (@ForN_ L G pb i n nocrash oncrash t0)
+  {{ loopvar ~> t0 * v ~> i * term ~> (i + n) * F }}
+    Go.While (TestE Lt (Var v) (Var term))
+      (xpb)
+  {{ fun ret => loopvar ~> ret * v ~> (i + n) * term ~> (i + n) * F }} // env.
+Proof.
+  induction n; intros; simpl.
+  - unfold ProgOk. intros.
+    rewrite <- plus_n_O in *.
+    repeat destruct_pair.
+    inv_exec.
+    + inv_exec.
+      eval_expr.
+      inv_exec_progok.
+    + inv_exec_progok.
+      contradiction H2.
+      repeat eexists.
+      eapply StepWhileFalse.
+      eval_expr.
+    + inv_exec_progok.
+  - unfold ProgOk. intros.
+    destruct_pairs.
+    destruct out.
+    + (* failure case *)
+      intuition try congruence.
+      inv_exec.
+      {
+        inv_exec; eval_expr.
+        find_eapply_lem_hyp ExecFailed_Steps. repeat deex.
+        find_eapply_lem_hyp Steps_Seq.
+        intuition subst; repeat deex.
+        { (* failure in body *)
+          eapply Prog.XBindFail.
+          repeat destruct_pair.
+          edestruct H; eauto.
+          2 : eapply Steps_ExecFailed; [> | | eauto].
+          pred_solve.
+          unfold is_final; simpl; intro; subst; eauto.
+          edestruct ExecFailed_Steps.
+          eapply Steps_ExecFailed; eauto.
+          eapply steps_sequence. eauto.
+          repeat deex; eauto.
+          intuition eauto.
+        }
+        { (* failure in loop *)
+          find_eapply_lem_hyp Steps_ExecFinished.
+          edestruct H; eauto. pred_cancel.
+          edestruct H4; eauto. simpl in *; repeat deex.
+          destruct_pair; simpl in *.
+          edestruct (IHn (S i));
+            [> | | eapply Steps_ExecFailed; eauto |];
+            rewrite ?plus_Snm_nSm; eauto.
+          intuition eauto.
+        }
+      }
+      {
+        contradiction H3.
+        repeat eexists.
+        eapply StepWhileTrue.
+        eval_expr.
+      }
+    + (* finished case *)
+      inv_exec. inv_exec; eval_expr. subst_definitions.
+      intuition try congruence. repeat find_inversion_safe.
+      repeat match goal with
+      | [H : context[Init.Nat.add _ (S _)] |- _] =>
+          (rewrite <- plus_Snm_nSm in H || setoid_rewrite <- plus_Snm_nSm in H)
+      end.
+      setoid_rewrite <- plus_Snm_nSm.
+      destruct_pairs.
+      find_eapply_lem_hyp ExecFinished_Steps.
+      find_eapply_lem_hyp Steps_Seq.
+      intuition; repeat deex; try discriminate.
+      repeat find_eapply_lem_hyp Steps_ExecFinished.
+      edestruct H; eauto; eauto.
+      forward_solve.
+      edestruct (IHn (S i)); eauto.
+      forward_solve.
+    + (* crashed case *)
+      intuition try congruence. find_inversion.
+      inv_exec; [> | solve [inversion H3] ].
+      inv_exec; eval_expr.
+      find_eapply_lem_hyp ExecCrashed_Steps.
+      intuition; repeat deex.
+      find_eapply_lem_hyp Steps_Seq.
+      intuition auto; repeat deex.
+      {
+        invc H4.
+        find_eapply_lem_hyp Steps_ExecCrashed; eauto.
+        edestruct H; forward_solve. auto.
+      }
+      {
+        find_eapply_lem_hyp Steps_ExecFinished.
+        find_eapply_lem_hyp Steps_ExecCrashed; eauto.
+        edestruct H; eauto. pred_cancel.
+        repeat match goal with
+        | [H : context[Init.Nat.add _ (S _)] |- _] =>
+            (rewrite <- plus_Snm_nSm in H || setoid_rewrite <- plus_Snm_nSm in H)
+        end.
+        edestruct H2; eauto.
+        forward_solve.
+        repeat deex.
+        edestruct IHn; eauto.
+        forward_solve.
+      }
+Qed.
+
+
+Lemma SetConstBefore : forall T (T' : GoWrapper T) (p : prog T) env xp v n A B,
+  EXTRACT p {{ v ~> n * A }} xp {{ B }} // env ->
+  EXTRACT p
+    {{ v ~>? nat * A }}
+      v <~const n; xp
+    {{ B }} // env.
+Proof.
+  eauto using CompileBefore, CompileConst'.
+Qed.
+
+Lemma CompileDup : forall env X (Wr : GoWrapper X) F (var var' : var) x,
+  EXTRACT Ret x
+  {{ var ~> x * var' ~>? X * F }}
+    var' <~dup var
+  {{ fun ret => var ~> x * var' ~> ret * F }} // env.
+Proof.
+  unfold ProgOk.
+  inv_exec_progok.
+  - repeat inv_exec.
+    eval_expr.
+    repeat econstructor.
+    pred_solve.
+  - repeat inv_exec.
+  - repeat inv_exec.
+    + exfalso; eauto.
+    + contradiction H1. eval_expr.
+      repeat econstructor;
+        [ eval_expr; eauto .. ].
+Qed.
+
+Lemma DuplicateBefore : forall T (T' : GoWrapper T) X (X' : GoWrapper X)
+  (p : prog T) xp env v v' (x x' : X) A B,
+  EXTRACT p {{ v ~> x * v' ~> x * A }} xp {{ B }} // env ->
+  EXTRACT p
+    {{ v ~> x' * v' ~> x * A }}
+      v <~dup v'; xp
+    {{ B }} // env.
+Proof.
+  unfold ProgOk.
+  inv_exec_progok.
+  - do 5 inv_exec. inv_exec.
+    eval_expr.
+    edestruct H; forward_solve.
+    simpl. pred_solve.
+  - do 5 inv_exec; try solve [inv_exec].
+    eval_expr.
+    edestruct H; forward_solve.
+    simpl. pred_solve.
+  - inv_exec.
+    do 3 inv_exec; forward_solve.
+    inv_exec. inv_exec.
+    eval_expr.
+    edestruct H; forward_solve.
+    simpl. pred_solve.
+    contradiction H2.
+    repeat eexists; eauto.
+    do 2 econstructor; solve [eval_expr; eauto].
+Qed.
+
+Lemma AddInPlaceLeftBefore : forall T (T' : GoWrapper T) (p : prog T) B xp env
+  va a v x F,
+  EXTRACT p {{ v ~> (x + a) * va ~> a * F }} xp {{ B }} // env ->
+  EXTRACT p
+  {{ v ~> x * va ~> a * F }}
+    Go.Modify (Go.ModifyNumOp Plus) (v, v, va); xp
+  {{ B }} // env.
+Proof.
+  intros.
+  eapply CompileBefore; eauto.
+  eapply hoare_weaken.
+  eapply CompileRet with (T := nat) (var0 := v).
+  eapply hoare_weaken_post; [ | eapply CompileAddInPlace1 with (avar := v) (bvar := va) ].
+  all : cancel_go.
+Qed.
+
+Lemma AddInPlaceLeftAfter : forall T (T' : GoWrapper T) (p : prog T) A xp env
+  va a v x F,
+  EXTRACT p {{ A }} xp {{ fun ret => F ret * v ~> x * va ~> a }} // env ->
+  EXTRACT p
+  {{ A }}
+    xp; Go.Modify (Go.ModifyNumOp Plus) (v, v, va)
+  {{ fun ret => F ret * v ~> (x + a) * va ~> a }} // env.
+Proof.
+  intros.
+  eapply CompileAfter; eauto.
+  intros.
+  eapply hoare_weaken_post; [ | eapply CompileRet with (var0 := v) (v := x + a) ].
+  cancel_go.
+  eapply hoare_weaken.
+  eapply CompileAddInPlace1 with (avar := v) (bvar := va).
+  all: cancel_go.
+Qed.
+
+Lemma CompileFor : forall L G (L' : GoWrapper L) loopvar F
+                          v vn (n i : W)
+                          t0 env (pb : W -> L -> prog L) xpb nocrash oncrash,
+    (forall t x v term one,
+        EXTRACT (pb x t)
+  {{ loopvar ~> t * v ~> x * term ~> (i + n) * one ~> 1 * vn ~> n * F }}
+    xpb v term one
+  {{ fun ret => loopvar ~> ret * v ~> x * term ~> (i + n) * one ~> 1 * vn ~> n * F }} // env)
+  ->
+  EXTRACT (@ForN_ L G pb i n nocrash oncrash t0)
+  {{ loopvar ~> t0 * v ~> i * vn ~> n * F }}
+    Declare Num (fun one => (
+      one <~const 1;
+      Declare Num (fun term => (
+        Go.Modify (Go.DuplicateOp) (term, v);
+        Go.Modify (Go.ModifyNumOp Go.Plus) (term, term, vn);
+        Go.While (TestE Lt (Var v) (Var term)) (
+          xpb v term one;
+          Go.Modify (Go.ModifyNumOp Go.Plus) (v, v, one)
+        )
+      ))
+    ))
+  {{ fun ret => loopvar ~> ret * v |->? * vn |->? * F }} // env.
+Proof.
+  intros.
+  eapply CompileDeclare with (Wr := GoWrapper_Num). intro one.
+  eapply hoare_strengthen_pre; [>
+  | eapply SetConstBefore; eauto ].
+  cancel_go.
+  eapply CompileDeclare with (Wr := GoWrapper_Num). intro term.
+  eapply hoare_strengthen_pre; [>
+  | eapply DuplicateBefore with (x' := 0) (x := i); eauto].
+  cancel_go.
+  eapply hoare_strengthen_pre; [>
+  | eapply AddInPlaceLeftBefore with (a := n) (x := i); eauto ].
+  cancel_go.
+  eapply hoare_strengthen_pre; [>
+  | eapply hoare_weaken_post; [>
+  | eapply CompileForLoopBasic with (t0 := t0) (loopvar := loopvar)] ].
+  cancel_go.
+  cancel_go.
+  intros.
+  eapply hoare_weaken_post; [>
+  | eapply AddInPlaceLeftAfter with (a := 1) (x := x); eauto].
+  rewrite Nat.add_1_r.
+  instantiate (1 := fun x0 => (loopvar ~> x0 * term ~> (i + n) * _)%pred).
+  cancel_go.
+  specialize (H t x v term one).
+  eapply hoare_strengthen_pre. shelve.
+  eapply hoare_weaken_post. shelve.
+  eauto.
+  Unshelve.
+  all : cancel_go.
+Qed.
+
+Definition voidfunc2 A B C {WA: GoWrapper A} {WB: GoWrapper B} name (src : A -> B -> prog C) env :=
+  forall avar bvar,
+    forall a b F, EXTRACT src a b
+           {{ avar ~> a * bvar ~> b * F }}
+             Call [] name [avar; bvar]
+           {{ fun _ => avar |->? * bvar |->? * F
+            (* TODO: could remember a & b if they are of aliasable type *) }} // env.
+
+
+(* TODO: generalize for all kinds of functions *)
+Lemma extract_voidfunc2_call :
+  forall A B C {WA: GoWrapper A} {WB: GoWrapper B} name (src : A -> B -> prog C) arga argb arga_t argb_t env,
+    forall and body ss,
+      (forall a b F, EXTRACT src a b {{ arga ~> a * argb ~> b * F }} body {{ fun _ => arga |->? * argb |->? * F }} // env) ->
+      StringMap.find name env = Some {|
+                                    ParamVars := [(arga_t, arga); (argb_t, argb)];
+                                    RetParamVars := [];
+                                    Body := body;
+                                    (* ret_not_in_args := rnia; *)
+                                    args_no_dup := and;
+                                    body_source := ss;
+                                  |} ->
+      voidfunc2 name src env.
+Proof.
+  unfold voidfunc2.
+  intros A B C WA WB name src arga argb arga_t argb_t env and body ss Hex Henv avar bvar a b F.
+  specialize (Hex a b F).
+  intro.
+  intros.
+  intuition subst.
+  - find_eapply_lem_hyp ExecFinished_Steps.
+    find_eapply_lem_hyp Steps_runsto.
+    invc H0.
+    find_eapply_lem_hyp runsto_Steps.
+    find_eapply_lem_hyp Steps_ExecFinished.
+    rewrite Henv in H4.
+    find_inversion_safe.
+    subst_definitions. unfold sel in *. simpl in *. unfold ProgOk in *.
+    repeat eforward Hex.
+    forward Hex.
+    shelve.
+    forward_solve.
+    simpl in *.
+    do 2 eexists.
+    intuition eauto.
+    break_match.
+    (*
+    eauto.
+
+    econstructor.
+    econstructor.
+  - find_eapply_lem_hyp ExecCrashed_Steps.
+    repeat deex.
+    invc H1; [ solve [ invc H2 ] | ].
+    invc H0.
+    rewrite Henv in H7.
+    find_inversion_safe. unfold sel in *. simpl in *.
+    assert (exists bp', (Go.step env)^* (d, callee_s, body) (final_disk, s', bp') /\ p' = InCall s [arga; argb] [] [avar; bvar] [] bp').
+    {
+      remember callee_s.
+      clear callee_s Heqt.
+      generalize H3 H2. clear. intros.
+      prep_induction H3; induction H3; intros; subst.
+      - find_inversion.
+        eauto using rt1n_refl.
+      - invc H0.
+        + destruct st'.
+          forwardauto IHclos_refl_trans_1n; deex.
+          eauto using rt1n_front.
+        + invc H3. invc H2. invc H.
+    }
+    deex.
+    eapply Steps_ExecCrashed in H1.
+    unfold ProgOk in *.
+    repeat eforward Hex.
+    forward Hex.
+    shelve.
+    forward_solve.
+    invc H2. trivial.
+  - find_eapply_lem_hyp ExecFailed_Steps.
+    repeat deex.
+    invc H1.
+    + contradiction H3.
+      destruct st'. repeat eexists. econstructor; eauto.
+      unfold sel; simpl in *.
+      maps.
+      find_all_cases.
+      trivial.
+    + invc H2.
+      rewrite Henv in H8.
+      find_inversion_safe. simpl in *.
+      assert (exists bp', (Go.step env)^* (d, callee_s, body) (st', bp') /\ p' = InCall s [arga; argb] [] [avar; bvar] [] bp').
+      {
+        remember callee_s.
+        clear callee_s Heqt.
+        generalize H4 H0 H3. clear. intros.
+        prep_induction H4; induction H4; intros; subst.
+        - find_inversion.
+          eauto using rt1n_refl.
+        - invc H0.
+          + destruct st'0.
+            forwardauto IHclos_refl_trans_1n; deex.
+            eauto using rt1n_front.
+          + invc H4. contradiction H1. auto. invc H.
+      }
+      deex.
+      eapply Steps_ExecFailed in H2.
+      unfold ProgOk in *.
+      repeat eforward Hex.
+      forward Hex. shelve.
+      forward_solve.
+      intuition.
+      contradiction H3.
+      unfold is_final in *; simpl in *; subst.
+      destruct st'. repeat eexists. eapply StepEndCall; simpl; eauto.
+      intuition.
+      contradiction H3.
+      repeat deex; eauto.
+
+  Unshelve.
+  * simpl in *.
+    maps.
+    find_all_cases.
+    find_inversion_safe.
+    maps.
+    find_all_cases.
+    find_inversion_safe.
+    eapply Forall_elements_remove_weaken.
+    eapply forall_In_Forall_elements.
+    intros.
+    destruct (Nat.eq_dec k argb).
+    subst. maps. find_inversion_safe.
+    find_copy_eapply_lem_hyp NoDup_bool_sound.
+    invc H.
+    assert (arga <> argb).
+    intro. subst. contradiction H2. constructor. auto.
+    maps.
+    intros. apply sumbool_to_bool_dec.
+    maps.
+  * (* argh *)
+    simpl in *.
+    subst_definitions.
+    maps.
+    find_all_cases.
+    find_inversion_safe.
+    maps.
+    eapply Forall_elements_remove_weaken.
+    eapply forall_In_Forall_elements.
+    intros.
+    destruct (Nat.eq_dec k argb).
+    subst. maps. find_inversion_safe.
+    find_copy_eapply_lem_hyp NoDup_bool_sound.
+    invc H.
+    assert (arga <> argb).
+    intro. subst. contradiction H8. constructor. auto.
+    find_cases avar s.
+    find_cases bvar s.
+    find_inversion_safe.
+    maps.
+    intros. apply sumbool_to_bool_dec.
+    maps.
+  * unfold sel in *; simpl in *.
+    subst_definitions.
+    simpl in *.
+    find_cases avar s.
+    find_cases bvar s.
+    find_inversion_safe.
+    maps.
+    rewrite He in *.
+    auto.
+    eapply Forall_elements_remove_weaken.
+    eapply forall_In_Forall_elements.
+    intros.
+    destruct (Nat.eq_dec k argb).
+    subst. maps. find_inversion_safe.
+    find_copy_eapply_lem_hyp NoDup_bool_sound.
+    invc H.
+    assert (arga <> argb).
+    intro. subst. contradiction H9. constructor. auto.
+    maps.
+    rewrite He0 in *. auto.
+    intros. apply sumbool_to_bool_dec.
+    maps.
+*)
+Admitted.
+
+Lemma CompileSplit :
+  forall env A B {HA: GoWrapper A} {HB: GoWrapper B} avar bvar pvar F (p : A * B),
+    EXTRACT Ret tt
+    {{ avar ~>? A * bvar ~>? B * pvar ~> p * F }}
+      Modify SplitPair (pvar, avar, bvar)
+    {{ fun _ => avar ~> fst p * bvar ~> snd p * pvar |-> moved_value (wrap p) * F }} // env.
+Proof.
+  intros; unfold ProgOk.
+  inv_exec_progok.
+  - repeat inv_exec.
+    eval_expr.
+    repeat econstructor.
+    pred_solve.
+  - inv_exec_progok.
+  - inv_exec_progok.
+    eval_expr.
+    contradiction H1.
+    repeat econstructor;
+    [ eval_expr; eauto ..].
+Qed.
+
+Lemma CompileFst :
+  forall env A B {HA: GoWrapper A} {HB: GoWrapper B} avar bvar pvar F (p : A * B),
+    EXTRACT Ret (fst p)
+    {{ avar ~>? A * bvar ~>? B * pvar ~> p * F }}
+      Modify SplitPair (pvar, avar, bvar)
+    {{ fun ret => avar ~> ret * bvar ~> snd p * pvar |-> moved_value (wrap p) * F }} // env.
+Proof.
+  intros; unfold ProgOk.
+  inv_exec_progok.
+  - repeat inv_exec.
+    repeat econstructor.
+    eval_expr.
+    pred_solve.
+  - inv_exec_progok.
+  - inv_exec_progok.
+    eval_expr.
+    contradiction H1.
+    repeat econstructor;
+    [ eval_expr; eauto ..].
+Qed.
+
+Lemma CompileSnd :
+  forall env A B {HA: GoWrapper A} {HB: GoWrapper B} avar bvar pvar F (p : A * B),
+    EXTRACT Ret (snd p)
+    {{ avar ~>? A * bvar ~>? B * pvar ~> p * F }}
+      Modify SplitPair (pvar, avar, bvar)
+    {{ fun ret => avar ~> fst p * bvar ~> ret * pvar |-> moved_value (wrap p) * F }} // env.
+Proof.
+  intros; unfold ProgOk.
+  inv_exec_progok.
+  - repeat inv_exec.
+    repeat econstructor.
+    eval_expr.
+    pred_solve.
+  - inv_exec_progok.
+  - inv_exec_progok.
+    eval_expr.
+    contradiction H1.
+    repeat econstructor;
+    [ eval_expr; eauto ..].
+Qed.
+
+Lemma CompileJoin :
+  forall env A B {HA: GoWrapper A} {HB: GoWrapper B} avar bvar pvar (a : A) (b : B) F,
+    EXTRACT Ret (a, b)
+    {{ avar ~> a * bvar ~> b * pvar ~>? (A * B)%type * F }}
+      Modify JoinPair (pvar, avar, bvar)
+    {{ fun ret => avar |-> moved_value (wrap a) * bvar |-> moved_value (wrap b) * pvar ~> ret * F }} // env.
+Proof.
+  intros; unfold ProgOk.
+  repeat inv_exec_progok.
+  - repeat inv_exec.
+    eval_expr.
+    repeat econstructor.
+    pred_solve.
+  - contradiction H1.
+    eval_expr.
+    repeat econstructor.
+    eval_expr; eauto.
+    eval_expr; eauto.
+    eval_expr; eauto.
+Qed.
+
+Hint Constructors source_stmt.
+
+Lemma CompileRetOptionSome : forall env B {HB: GoWrapper B} {D : DefaultValue B}
+  avar bvar pvar (b : B) (p : bool * B) F,
+  EXTRACT Ret (Some b)
+  {{ avar ~> true * bvar ~> b * pvar ~> p * F }}
+    Modify JoinPair (pvar, avar, bvar)
+  {{ fun ret => pvar ~> ret *
+                avar |-> moved_value (wrap true) *
+                bvar |-> moved_value (wrap b) * F }} // env.
+Proof.
+  intros.
+  unfold ProgOk.
+  inv_exec_progok.
+  - repeat inv_exec.
+    repeat econstructor.
+    eval_expr.
+    pred_solve.
+  - inv_exec_progok.
+  - inv_exec_progok.
+    contradiction H1.
+    repeat econstructor;
+    [ eval_expr; eauto..].
+Qed.
+
+Lemma option_none_okToUnify : forall AT AEQ {T} {HT : GoWrapper T} {D : DefaultValue T} var,
+  @okToUnify AT AEQ value (var ~> None) (var |-> Val (Pair Bool wrap_type) (false, wrap' zeroval)).
+Proof.
+  intros.
+  unfold wrap. simpl.
+  rewrite default_zero' by apply default_zero.
+  reflexivity.
+Qed.
+
+Local Hint Extern 1 (okToUnify (?var ~> None)
+  (?var |-> Val (Pair Bool wrap_type) (false, wrap' zeroval)))
+  => apply option_none_okToUnify.
+
+Lemma CompileRetOptionNone : forall env B {HB: GoWrapper B} {D : DefaultValue B}
+  avar pvar (p : bool * B) F,
+  EXTRACT Ret None
+  {{ avar ~> false * pvar ~> p * F }}
+    Declare wrap_type (fun bvar =>
+      Modify JoinPair (pvar, avar, bvar)
+    )
+  {{ fun ret => pvar ~> ret *
+                avar |-> moved_value (wrap false) * F }} // env.
+Proof.
+  intros.
+  eapply CompileDeclare. intro bvar.
+  unfold ProgOk.
+  inv_exec_progok.
+  - repeat inv_exec.
+    repeat econstructor.
+    eval_expr.
+    pred_solve.
+    eapply pimpl_apply.
+    2: eapply ptsto_upd. 2: pred_apply; cancel_go. cancel_go.
+  - inv_exec_progok.
+  - inv_exec_progok.
+    contradiction H1.
+    repeat econstructor;
+    [ eval_expr; eauto..].
+Qed.
+
+Lemma CompileMatchOption : forall env B {HB : GoWrapper B} X {HX : GoWrapper X} {D : DefaultValue B}
+  ovar avar bvar xvar (o : option B)
+  (pnone : prog X) xpnone (psome : B -> prog X) xpsome (F : pred) C,
+  (forall (b : B),
+  EXTRACT (psome b)
+  {{ avar ~> true * bvar ~> b * ovar |-> moved_value (wrap o) * F }}
+    xpsome
+  {{ fun ret => xvar ~> ret * avar ~>? bool * bvar ~>? B * ovar ~>? option B * C }} // env) ->
+  EXTRACT pnone
+  {{ avar ~> false * bvar ~> zeroval * ovar |-> moved_value (wrap o) * F }}
+    xpnone
+  {{ fun ret => xvar ~> ret * avar ~>? bool * bvar ~>? B * ovar ~>? option B * C }} // env ->
+  EXTRACT (match o with
+           | None => pnone
+           | Some b => psome b
+           end)
+  {{ ovar ~> o * avar ~>? bool * bvar ~>? B * F }}
+    Modify SplitPair (ovar, avar, bvar) ;
+    If Var avar Then xpsome Else xpnone EndIf
+  {{ fun ret => xvar ~> ret * avar ~>? bool * bvar ~>? B * ovar ~>? option B * C }} // env.
+Proof.
+  intros.
+  eapply extract_equiv_prog with (pr1 := Bind (Ret tt) (fun _ => _)).
+  rewrite bind_left_id. apply prog_equiv_equivalence.
+  eapply CompileSeq.
+  {
+    eapply hoare_strengthen_pre;
+    [ | eapply CompileSplit with (p := match o with
+                                       | None => (false, zeroval)
+                                       | Some b => (true, b)
+                                       end)].
+    destruct o; simpl. cancel_go.
+    unfold wrap. simpl.
+    erewrite <- default_zero' by apply default_zero. cancel_go.
+  }
+  destruct o; simpl in *.
+  + unfold ProgOk; inv_exec_progok.
+    - inv_exec.
+      inv_exec; eval_expr.
+      edestruct H; eauto.
+      simpl. pred_solve.
+      forward_solve.
+    - inv_exec; inv_exec; eval_expr.
+      edestruct H; eauto.
+      simpl. pred_solve.
+      forward_solve.
+    - inv_exec.
+      inv_exec; eval_expr.
+      edestruct H; eauto.
+      simpl. pred_solve.
+      forward_solve.
+      contradiction H3.
+      repeat eexists. apply StepIfTrue. eval_expr.
+  + erewrite <- default_zero' in * by apply default_zero.
+    unfold ProgOk; inv_exec_progok.
+    - inv_exec.
+      inv_exec; eval_expr.
+      edestruct H0; eauto.
+      simpl. pred_solve.
+      forward_solve.
+    - inv_exec; inv_exec; eval_expr.
+      edestruct H0; eauto.
+      simpl. pred_solve.
+      forward_solve.
+    - inv_exec.
+      inv_exec; eval_expr.
+      edestruct H0; eauto.
+      simpl. pred_solve.
+      forward_solve.
+      contradiction H3.
+      repeat eexists. apply StepIfFalse. eval_expr.
+Qed.
