src/GoExtracted.v
@@ -1,0 +1,181 @@
+Require Import List String.
+Require Import StringMap.
+Require Import Word Prog Pred SepAuto.
+Require Import GoSemantics GoFacts GoHoare GoCompilationLemmas GoExtraction GoTactics2.
+Import ListNotations.
+Import Go.
+
+Open Scope pred_scope.
+
+Require Import Cache.
+
+Instance WrapByTransforming_cachestate : WrapByTransforming cachestate.
+  refine {|
+    transform := fun cs => (CSMap cs, CSMaxCount cs, CSEvict cs);
+  |}.
+  simpl; intros. repeat find_inversion_safe. destruct t1, t2; f_equal; auto.
+Defined.
+
+Instance cachestate_default_value : DefaultValue cachestate := {| zeroval :=
+  {| CSMap := Go.Map.empty _; CSMaxCount := 0; CSEvict := tt |} |}.
+  unfold wrap, wrap', GoWrapper_transform, default_value. simpl.
+  repeat f_equal.
+  apply MapUtils.addrmap_equal_eq.
+  apply MapUtils.AddrMap.map_empty.
+  auto with map.
+Defined.
+
+Instance addrmap_default_value : forall T {H: GoWrapper T}, DefaultValue (Map.t T).
+  intros.
+  apply Build_DefaultValue with (zeroval := Map.empty _).
+  unfold default_value, default_value', wrap, wrap'.
+  simpl. repeat f_equal.
+  apply MapUtils.addrmap_equal_eq.
+  apply MapUtils.AddrMap.map_empty.
+  eauto with map.
+Defined.
+
+Example compile_writeback : forall env, sigT (fun p => forall a cs,
+  EXTRACT BUFCACHE.writeback a cs
+  {{ 0 ~> a * 1 ~> cs }}
+    p
+  {{ fun ret => 0 |->? * 1 ~> ret }} // env).
+Proof.
+  unfold BUFCACHE.writeback.
+  intros.
+  compile_step.
+  eapply hoare_strengthen_pre.
+  rewrite transform_pimpl. simpl. reflexivity. (* TODO *)
+  compile_step.
+  compile_step.
+  compile_step.
+  compile_step.
+  compile_step.
+  compile_step.
+  compile_step.
+  compile_step.
+  compile_step.
+  compile_step.
+  compile_step.
+  compile_step.
+  compile_step.
+  compile_step.
+  compile_step.
+  compile_step.
+  compile_step.
+  3: cancel_go.
+  Focus 3. unfold exis'. cancel.
+  match goal with
+  | [ |- ?P =p=> ?Q ] => set Q
+  end.
+  pattern x in p. subst p. reflexivity.
+  compile_step.
+  compile_step.
+  compile_step.
+  compile_step.
+  compile_step.
+  (* TODO do the right thing here in compile_map_op *)
+  eapply CompileRet with (v := (CSMap cs)) (var0 := (snd (fst (fst (fst (fst (fst (fst (fst (fst (fst vars))))))))))).
+  compile_step.
+  compile_step.
+  compile_step.
+  compile_step. (* TODO rule for Ret false *)
+  {
+    eapply hoare_weaken.
+    eapply CompileRet', CompileSkip.
+    cancel_go. cancel_go.
+  }
+  compile_step.
+  compile_step.
+  eapply hoare_weaken.
+  eapply CompileRet' with (var0 := 1).
+  eapply hoare_weaken_post.
+  intros.
+  match goal with
+  | [ |- ?P =p=> ?Q ] => set (P)
+  end.
+  rewrite transform_pimpl. simpl.
+  subst p.
+  match goal with
+  | [ |- ?e _ =p=> ?Q ] => unify e (fun x : unit => Q)
+  end. reflexivity.
+  2: cancel_go.
+  2: cancel_go.
+  eapply CompileRet.
+  unfold prod'. (* TODO: prod' should never escape to this point! *)
+  compile_step.
+  compile_step.
+  compile_step.
+  eapply hoare_weaken.
+  eapply CompileRet' with (var0 := 1).
+  eapply hoare_weaken_post.
+  intros.
+  match goal with
+  | [ |- ?P =p=> ?Q ] => set (P)
+  end.
+  rewrite transform_pimpl. simpl.
+  subst p.
+  match goal with
+  | [ |- ?e _ =p=> ?Q ] => unify e (fun x : unit => Q)
+  end. reflexivity.
+  2: cancel_go.
+  2: cancel_go.
+  eapply CompileRet.
+  unfold prod'.
+  compile_step.
+  compile_step.
+  (***********)
+  (* This [compile_step] takes >2 minutes *)
+  (***********)
+  Time compile_step.
+  unfold exis'. cancel.
+  Axiom admit : False.
+  (* TODO: [CSMap cs] is gone! *) exfalso; apply admit.
+  eapply hoare_weaken.
+  eapply CompileRet' with (var0 := 1).
+  eapply hoare_weaken_post.
+  intros.
+  match goal with
+  | [ |- ?P =p=> ?Q ] => set (P)
+  end.
+  rewrite transform_pimpl. simpl.
+  subst p.
+  match goal with
+  | [ |- ?e _ =p=> ?Q ] => unify e (fun x : unit => Q)
+  end. reflexivity.
+  2: cancel_go.
+  2: cancel_go.
+  eapply CompileRet.
+  unfold prod'.
+  compile_step.
+  compile_step.
+  (* [compile_step] here works but takes >15 minutes... *)
+  match goal with
+  | |- EXTRACT Ret (?a_, ?b_)
+       {{ ?pre }}
+          _
+       {{ ?post }} // _ =>
+        match find_val a_ pre with
+        | Some ?ka =>
+            match find_val b_ pre with
+            | Some ?kb =>
+                match var_mapping_to_ret with
+                | ?kp =>
+                    eapply hoare_weaken;
+                     [ apply CompileJoin with
+                         (avar := ka) (bvar := kb) (pvar := kp)
+                     | .. ]
+                end
+            end
+        end
+  end.
+  simpl in *. fold prod' in *. cancel.
+  simpl in *. unfold exis' in *. cancel.
+  (* TODO: [CSMap cs] is gone! *) exfalso; apply admit.
+
+  Unshelve.
+  all: repeat constructor.
+  exact $0.
+(* This eats memory and dies: *)
+Defined.
+Eval lazy in (projT1_sig compile_writeback).
