src/GoExtraction.v
@@ -1,0 +1,468 @@
+Require Import ProofIrrelevance.
+Require Import Eqdep_dec.
+Require Import PeanoNat String List.
+Require Import Relation_Operators Operators_Properties.
+Require Import Morphisms.
+Require Import VerdiTactics.
+Require Import Word Mem AsyncDisk Pred PredCrash Prog ProgMonad SepAuto.
+Require Import BasicProg.
+Require Import Gensym.
+Require Import Omega.
+Require Import GoSemantics.
+Require Import GoFacts GoHoare GoTactics2 GoCompilationLemmas.
+
+Import ListNotations.
+
+Set Implicit Arguments.
+
+(* Don't print (elt:=...) everywhere *)
+Unset Printing Implicit Defensive.
+
+Definition extract_code := projT1.
+
+
+Local Open Scope pred.
+
+Import Go.
+
+Ltac find_val v p :=
+  match p with
+    | context[?k ~> v] => constr:(Some k)
+    | _ => constr:(@None var)
+  end.
+
+Ltac find_val_fn v p cont :=
+  match p with
+    | context[?k ~> v] => cont k
+  end.
+
+Ltac var_mapping_to pred val :=
+  lazymatch pred with
+    | context[?var ~> val] => var
+  end.
+
+Definition mark_ret (T : Type) := T.
+Class find_ret {T} (P : pred) := FindRet : T.
+Ltac find_ret_tac P :=
+  match goal with
+    | [ ret : mark_ret ?T |- _ ] => var_mapping_to P ret
+  end.
+Hint Extern 0 (@find_ret ?T ?P) => (let x := find_ret_tac P in exact x) : typeclass_instances.
+Ltac var_mapping_to_ret :=
+  lazymatch goal with
+    | [ |- EXTRACT _ {{ _ }} _ {{ fun ret : ?T => ?P }} // _ ] =>
+      lazymatch constr:(fun ret : mark_ret T => (_:find_ret P)) with
+        | (fun ret => ?var) => var
+      end
+  end.
+
+Ltac do_declare T cont :=
+  lazymatch goal with
+  | [ |- EXTRACT _ {{ ?pre }} _ {{ _ }} // _ ] =>
+    lazymatch pre with
+    | context [decls_pre ?decls ?vars] =>
+      let decls' := fresh "decls" in
+      evar (decls' : list Declaration);
+      unify decls (Decl T :: decls'); subst decls';
+      cont (@snd (n_tuple_unit
+        (@Datatypes.length _ _) _) _ vars)
+    end
+  end.
+
+Ltac compile_bind := match goal with
+  | [ |- EXTRACT Bind ?p (fun _ => ?q) {{ _ }} _ {{ _ }} // _ ] =>
+    eapply CompileSeq
+  | [ |- EXTRACT Bind (Ret ?x_) ?p {{ _ }} _ {{ ?post }} // _ ] =>
+    match type of x_ with
+    | ?T_ =>
+      let Wr_ := constr:(ltac:(eauto with typeclass_instances) : GoWrapper T_) in
+      do_declare T_ ltac:(fun v_ =>
+        eapply hoare_strengthen_pre; [
+        | eapply CompileBindRet with (vara := v_) (a := x_)];
+        [ cancel_go | ..])
+    end
+  | [ |- EXTRACT Bind ?p ?q {{ _ }} _ {{ ?post }} // _ ] =>
+    match type of p with
+    | prog ?T_ =>
+      let v := fresh "var" in
+      let Wr_ := constr:(ltac:(eauto with typeclass_instances) : GoWrapper T_) in
+      do_declare T_ ltac:(fun v_ =>
+        simpl decls_pre; simpl decls_post;
+        match goal with [ |- EXTRACT _ {{ _ }} _ {{ ?post' }} // _ ] =>
+          simpl decls_post; simpl decls_pre;
+          eapply hoare_strengthen_pre;
+          [| eapply CompileBind with (var0 := v_)];
+          [ cancel_go | intros .. ]
+        end)
+    end
+  end.
+
+Ltac compile_const :=
+  lazymatch goal with
+  | [ |- EXTRACT Ret ?n {{ _ }} _ {{ _ }} // _] =>
+    match goal with
+    | [ x : _ |- _] =>
+      lazymatch n with
+      | context [x] => fail 1
+      end
+      | _ => idtac
+    end;
+      match var_mapping_to_ret with
+      | ?x => eapply hoare_weaken;
+        [eapply CompileConst with (var0 := x) | cancel_go..]
+      end
+  end.
+
+Ltac compile_ret := match goal with
+  | [ |- EXTRACT Ret tt {{ _ }} _ {{ _ }} // _ ] =>
+    eapply hoare_weaken_post; [ | eapply CompileSkip ]; [ cancel_go ]
+  | [ |- EXTRACT Ret ?x {{ ?pre }} _ {{ _ }} // _ ] =>
+    match find_val x pre with
+    | Some ?kx =>
+      match var_mapping_to_ret with
+      | ?kret => (unify kx kret; fail 2) ||
+        eapply hoare_weaken; [
+        eapply CompileDup with (var0 := kx) (var' := kret)
+        | cancel_go.. ]
+      end
+    end
+  end.
+
+Ltac compile_match := match goal with
+  | [ |- EXTRACT match ?o with _ => _ end {{ ?pre }} _ {{ fun ret => ?post }} // _ ] =>
+    match type of o with
+    | option ?X =>
+      match find_val o pre with
+      | None =>
+        eapply extract_equiv_prog with (pr1 := Bind (Ret o) (fun x => _));
+        [ generalize o; intro; rewrite bind_left_id; apply prog_equiv_equivalence |]
+      | Some ?x =>
+        match var_mapping_to_ret with
+        | ?ret =>
+          do_declare bool ltac:(fun vara => simpl decls_pre; simpl decls_post;
+            do_declare X ltac:(fun varb =>
+              eapply hoare_weaken;
+              [ eapply CompileMatchOption with
+                  (ovar := x) (avar := vara) (bvar := varb) (xvar := ret) | cancel_go.. ];
+              intros
+            ))
+        end
+      end
+    end
+  | [|- EXTRACT (let (a_, b_) := ?p in _) {{ _ }} _ {{ _ }} // _ ] =>
+    let H := fresh "H" in
+    let a := fresh "p" in
+    let b := fresh "p" in
+    destruct p as [a  b] eqn:H;
+    assert (a = fst p) by (subst p; eauto);
+    assert (b = snd p) by (subst p; eauto);
+    clear H; subst a b
+  end.
+
+Ltac compile_read_write := match goal with
+  | [ |- EXTRACT Read ?a {{ ?pre }} _ {{ _ }} // _ ] =>
+    let retvar := var_mapping_to_ret in
+    match find_val a pre with
+    | Some ?k =>
+      eapply hoare_strengthen_pre; [| eapply hoare_weaken_post; [ |
+        eapply CompileRead with (avar := k) (vvar := retvar) ] ]; [ cancel_go .. ]
+    end
+  | [ |- EXTRACT Write ?a ?v {{ ?pre }} _ {{ _ }} // _ ] =>
+    match find_val a pre with
+    | Some ?ka =>
+      match find_val v pre with
+      | Some ?kv =>
+        eapply hoare_strengthen_pre; [ | eapply hoare_weaken_post; [ |
+          eapply CompileWrite with (avar := ka) (vvar := kv) ] ]; [ cancel_go .. ]
+      end
+    end
+  end.
+
+Ltac compile_for := match goal with
+  | [ |- EXTRACT ForN_ ?f ?i ?n _ _ ?t0 {{ ?pre }} _ {{ _ }} // _ ] =>
+    let retvar := var_mapping_to_ret in
+    match find_val n pre with
+      | None => eapply extract_equiv_prog with (pr1 := Bind (Ret n) (fun x => ForN_ f i x _ _ t0));
+          [> rewrite bind_left_id; eapply prog_equiv_equivalence | ]
+      | Some ?kn =>
+      match find_val i pre with
+        | None => eapply extract_equiv_prog with (pr1 := Bind (Ret i) (fun x => ForN_ f x n _ _ t0));
+          [> rewrite bind_left_id; eapply prog_equiv_equivalence | ]
+        | Some ?ki =>
+        match find_val t0 pre with
+          | None => eapply extract_equiv_prog with (pr1 := Bind (Ret t0) (fun x => ForN_ f i n _ _ x));
+            [> rewrite bind_left_id; eapply prog_equiv_equivalence | ]
+          | Some ?kt0 =>
+            eapply hoare_strengthen_pre; [>
+            | eapply hoare_weaken_post; [>
+            | eapply CompileFor with (v := ki) (loopvar := kt0) (vn := kn)] ];
+            [> cancel_go | cancel_go | intros ]
+        end
+      end
+    end
+  end.
+
+Ltac compile_call := match goal with
+  | [ H : voidfunc2 ?name ?f ?env |- EXTRACT ?f ?a ?b {{ ?pre }} _ {{ _ }} // ?env ] =>
+    match find_val a pre with
+      | Some ?ka =>
+        match find_val b pre with
+          | Some ?kb =>
+            eapply hoare_weaken_post; [ | eapply hoare_strengthen_pre; [ |
+              eapply H with (avar := ka) (bvar := kb) ] ]; [ cancel_go .. ]
+        end
+    end
+  end.
+
+Ltac compile_add := match goal with
+  | [ |- EXTRACT Ret (S ?a) {{ ?pre }} _ {{ _ }} // _ ] =>
+    rewrite <- (Nat.add_1_r a)
+  | [ |- EXTRACT Ret (?a + ?b) {{ ?pre }} _ {{ _ }} // _ ] =>
+    let retvar := var_mapping_to_ret in
+    match find_val a pre with
+      | Some ?ka =>
+        match find_val b pre with
+          | Some ?kb =>
+            eapply hoare_weaken;
+              [ (unify retvar ka; eapply CompileAddInPlace1 with (avar := ka) (bvar := kb)) ||
+                (unify retvar kb; eapply CompileAddInPlace2 with (avar := ka) (bvar := kb)) ||
+                eapply CompileAdd with (avar := ka) (bvar := kb) (sumvar := retvar) | .. ];
+            [ cancel_go .. ]
+        end
+    end
+  end.
+
+Ltac compile_listop := match goal with
+  | [ |- EXTRACT Ret (?x :: ?xs) {{ ?pre }} _ {{ _ }} // _ ] =>
+    match find_val x pre with
+      | Some ?kx =>
+        match var_mapping_to_ret with
+          | ?kret =>
+            match find_val xs pre with
+              | Some ?kxs => (* ret var is tail var *)
+                unify kret kxs;
+                eapply hoare_weaken;
+                [ eapply CompileAppend with (lvar := kxs) (vvar := kx)
+                | cancel_go..]
+              | Some ?kxs => (* ret var is not tail var *)
+                eapply CompileBefore; [
+                  eapply CompileRet with (v := xs) (var0 := kret);
+                    simpl decls_pre |]
+            end
+        end
+    end
+  end.
+
+Ltac compile_map_op := match goal with
+  | [ |- EXTRACT Ret (Map.find ?k ?m) {{ ?pre }} _ {{ fun ret : ?T => ?post }} // _ ] =>
+    match find_val k pre with
+    | Some ?vark =>
+      match find_val m pre with
+      | Some ?varm =>
+        match var_mapping_to_ret with
+        | ?ret =>
+          eapply hoare_weaken; [
+          eapply CompileMapFind with (mvar := varm) (kvar := vark) (vvar := ret) | cancel_go..]
+        end
+      end
+    end
+  | [ |- EXTRACT Ret (Map.add ?k ?v ?m) {{ ?pre }} _ {{ fun ret : ?T => ?post }} // _ ] =>
+    match var_mapping_to_ret with
+    | ?retv =>
+      match find_val m pre with
+      | Some ?varm => unify retv varm; (* same variable *)
+        match find_val k pre with
+        | Some ?vark =>
+          match find_val v pre with
+          | Some ?varv =>
+            eapply hoare_weaken; [
+            eapply CompileMapAdd with (kvar := vark) (vvar := varv) (mvar := varm) |
+            cancel_go..]
+          end
+        end
+      | Some ?varm => (* not the same variable *)
+        (unify retv varm; fail 2) ||
+        eapply CompileBefore; [
+        idtac m retv "TODO apply CompileRet"
+        (* TODO apply CompileRet *)
+        |]
+      end
+    end
+  | [ |- EXTRACT Ret (Map.remove ?k ?m) {{ ?pre }} _ {{ fun ret : ?T => ?post }} // _ ] =>
+    match find_val k pre with
+    | Some ?vark =>
+      match find_val m pre with
+      | Some ?varm =>
+        eapply hoare_weaken; [
+        eapply CompileMapRemove with (kvar := vark) (mvar := varm) |
+        cancel_go..]
+      end
+    end
+  end.
+
+Ltac in_pair v pair path :=
+  match pair with
+  | v => constr:(Some path)
+  | (?a, ?b) =>
+    match in_pair v a (fst path) with
+    | Some ?x => constr:(Some x)
+    | None =>
+      match in_pair v b (snd path) with
+      | Some ?x => constr:(Some x)
+      | None => constr:(@None unit)
+      end
+    end
+  | _ => constr:(@None unit)
+  end.
+
+Ltac find_pair_val v p :=
+  match p with
+  | context [?k ~> ?v0] =>
+    match in_pair v v0 v0 with
+    | Some ?x => constr:(Some (k, x))
+    end
+  | _ => constr:(@None unit)
+  end.
+
+
+Ltac compile_split := match goal with
+  | [ |- EXTRACT Ret ?a {{ ?pre }} _ {{ _ }} // _ ] =>
+    match find_pair_val a pre with
+    | Some (_, ?ppath) =>
+      change (Ret a) with (Ret ppath)
+    end
+  | [ |- EXTRACT Ret (fst ?p) {{ ?pre }} _ {{ _ }} // _ ] =>
+    let avar_ := var_mapping_to_ret in
+    match find_val p pre with
+    | Some ?pvar_ =>
+      let A_ := type of (fst p) in
+      let B_ := type of (snd p) in
+      do_declare B_ ltac:(fun bvar_ =>
+        eapply hoare_weaken;
+        [ eapply CompileFst with (A := A_) (B := B_) (avar := avar_) (bvar := bvar_) (pvar := pvar_)
+        | cancel_go.. ])
+    end
+  | [ |- EXTRACT Ret (snd ?p) {{ ?pre }} _ {{ _ }} // _ ] =>
+    let bvar_ := var_mapping_to_ret in
+    match find_val p pre with
+    | Some ?pvar_ =>
+      let A_ := type of (fst p) in
+      let B_ := type of (snd p) in
+      do_declare A_ ltac:(fun avar_ =>
+        eapply hoare_weaken;
+        [ eapply CompileSnd with (A := A_) (B := B_) (avar := avar_) (bvar := bvar_) (pvar := pvar_)
+        | cancel_go.. ])
+    end
+  end.
+
+Ltac compile_join := match goal with
+  | [ |- EXTRACT Ret (?a_, ?b_) {{ ?pre }} _ {{ ?post }} // _ ] =>
+    match find_val a_ pre with
+    | None =>
+      let A_ := type of a_ in
+      eapply CompileBefore; [
+        do_declare A_ ltac:(fun x_ =>
+          eapply CompileRet with (v := a_) (var0 := x_);
+          simpl decls_pre) |]
+    | Some ?ka =>
+      match find_val b_ pre with
+      | None =>
+        let B_ := type of b_ in
+        eapply CompileBefore; [
+          do_declare B_ ltac:(fun x_ =>
+          eapply CompileRet with (v := b_) (var0 := x_);
+          simpl decls_pre) |]
+      | Some ?kb =>
+        match var_mapping_to_ret with
+        | ?kp =>
+          eapply hoare_weaken;
+          [ apply CompileJoin with (avar := ka) (bvar := kb) (pvar := kp)
+          | cancel_go..]
+        end
+      end
+    end
+end.
+
+Ltac compile_decompose := match goal with
+  | [ |- EXTRACT Ret (?f ?a) {{ ?pre }} _ {{ _ }} // _ ] =>
+    match find_val a pre with
+      | None =>
+        eapply extract_equiv_prog; [
+            let arg := fresh "arg" in
+            set (arg := Ret (f a));
+            pattern a in arg; subst arg;
+            eapply bind_left_id | ]
+    end
+   | [ |- EXTRACT Ret (?f ?a ?b) {{ ?pre }} _ {{ _ }} // _ ] =>
+    match find_val a pre with
+      | None => 
+        eapply extract_equiv_prog; [
+            let arg := fresh "arg" in
+            set (arg := Ret (f a b));
+            pattern a in arg; subst arg;
+            eapply bind_left_id | ]
+    end
+   | [ |- EXTRACT Ret (?f ?a ?b ?c) {{ ?pre }} _ {{ _ }} // _ ] =>
+    match find_val a pre with
+      | None =>
+        eapply extract_equiv_prog; [
+            let arg := fresh "arg" in
+            set (arg := Ret (f a b c));
+            pattern a in arg; subst arg;
+            eapply bind_left_id | ]
+    end
+  | [ |- EXTRACT ?f ?a {{ ?pre }} _ {{ _ }} // _ ] =>
+    match f with
+      | Ret => fail 2
+      | _ => idtac
+    end;
+    match find_val a pre with
+      | None =>
+        eapply extract_equiv_prog; [ eapply bind_left_id | ]
+    end
+  | [ |- EXTRACT ?f ?a ?b {{ ?pre }} _ {{ _ }} // _ ] =>
+    match find_val a pre with
+    | None =>
+      eapply extract_equiv_prog; [
+        let arg := fresh "arg" in
+        set (arg := f a b);
+        pattern a in arg; subst arg;
+        eapply bind_left_id | ]
+    end
+  end.
+
+Ltac compile_if := match goal with
+  | [|- EXTRACT (if ?x_ then _ else _) {{ ?pre }} _ {{ _ }} // _ ] =>
+    match find_val x_ pre with
+    | None =>
+      eapply extract_equiv_prog with (pr1 := Bind (Ret x_) (fun x => if x then _ else _));
+      [ rewrite bind_left_id; apply prog_equiv_equivalence |]
+    | Some ?kx_ =>
+      eapply hoare_weaken; [eapply CompileIf with (varb := kx_)|
+      cancel_go..]
+    end
+  end.
+
+Ltac compile_step :=
+  match goal with
+  | [ |- @sigT _ _ ] => eexists; intros; eapply CompileDeclareMany; intro
+  | _ => eapply decls_pre_impl_post
+  end
+  || compile_bind
+  || compile_const
+  || compile_ret
+  || compile_match
+  || compile_read_write
+  || compile_if
+  || compile_for
+  || compile_call
+  || compile_add
+  || compile_listop
+  || compile_map_op
+  || compile_join
+  || compile_split
+  || compile_decompose
+  .
+
+Ltac compile :=
+  unshelve (repeat compile_step); try exact nil.
