src/GoFacts.v
@@ -1,0 +1,346 @@
+Require Import List PeanoNat.
+Require Import Omega.
+Require Import Structures.OrderedTypeEx.
+Require Import Mem AsyncDisk Pred PredCrash ProgMonad SepAuto.
+Require Import GoTactics2.
+Require Import GoHoare.
+Require Import GoSemantics.
+Require Import StringMap MoreMapFacts.
+
+Set Implicit Arguments.
+
+Module VarMapFacts := FMapFacts.WFacts_fun(Nat_as_OT)(VarMap).
+Module Import MoreVarMapFacts := MoreFacts_fun(Nat_as_OT)(VarMap).
+
+Notation "k -s> v ;  m" := (StringMap.add k v m) (at level 21, right associativity) : map_scope.
+Delimit Scope map_scope with map.
+
+Notation "k ->> v ;  m" := (VarMap.add k v m) (at level 21, right associativity) : map_scope.
+
+
+Lemma possible_sync_refl : forall AT AEQ (m: @mem AT AEQ _), possible_sync m m.
+Proof.
+  intros.
+  unfold possible_sync.
+  intros.
+  destruct (m a).
+  destruct p.
+  right. repeat eexists. unfold incl. eauto.
+  eauto.
+Qed.
+
+Hint Immediate possible_sync_refl.
+
+Lemma read_fails_not_present:
+  forall env vvar avar (a : W) (v0 : valu) d s,
+    VarMap.find avar s = Some (wrap a) ->
+    VarMap.find vvar s = Some (wrap v0) ->
+    ~ (exists st' p', Go.step env (d, s, Go.DiskRead vvar (Go.Var avar)) (st', p')) ->
+    d a = None.
+Proof.
+  intros.
+  assert (~exists v0, d a = Some v0).
+  intuition.
+  deex.
+  contradiction H1.
+  destruct v1. repeat eexists. econstructor; eauto.
+  destruct (d a); eauto. contradiction H2. eauto.
+Qed.
+Hint Resolve read_fails_not_present.
+
+Lemma write_fails_not_present:
+  forall env vvar avar (a : W) (v : valu) d s,
+    VarMap.find vvar s = Some (wrap v) ->
+    VarMap.find avar s = Some (wrap a) ->
+    ~ (exists st' p', Go.step env (d, s, Go.DiskWrite (Go.Var avar) (Go.Var vvar)) (st', p')) ->
+    d a = None.
+Proof.
+  intros.
+  assert (~exists v0, d a = Some v0).
+  intuition.
+  deex.
+  contradiction H1.
+  destruct v0. repeat eexists. econstructor; eauto.
+  destruct (d a); eauto. contradiction H2. eauto.
+Qed.
+Hint Resolve write_fails_not_present.
+
+Lemma skip_is_final :
+  forall d s, Go.is_final (d, s, Go.Skip).
+Proof.
+  unfold Go.is_final; trivial.
+Qed.
+
+Hint Resolve skip_is_final.
+
+Definition vars_subset V (subset set : VarMap.t V) := forall k, VarMap.find k set = None -> VarMap.find k subset = None.
+
+Definition list_max l := fold_left max l 0.
+
+Theorem le_fold_max : forall l v,
+  v <= fold_left Init.Nat.max l v.
+Proof.
+  induction l; auto.
+  simpl; intros.
+  let HH := fresh in (edestruct Max.max_dec as [HH | HH]; rewrite HH).
+  eauto.
+  eapply le_trans.
+  apply Nat.max_r_iff; eauto.
+  eauto.
+Qed.
+
+Theorem le_fold_max_trans : forall l a b,
+  a <= b ->
+  fold_left Init.Nat.max l a <= fold_left Init.Nat.max l b.
+Proof.
+  induction l; intros. auto.
+  simpl.
+  repeat (let HH := fresh in (edestruct Max.max_dec as [HH | HH]; rewrite HH));
+  repeat rewrite ?Nat.max_l_iff, ?Nat.max_r_iff in *;
+  intuition.
+Qed.
+
+Theorem gt_list_max : forall l v,
+  v > list_max l ->
+  ~ In v l.
+Proof.
+  unfold list_max.
+  induction l; intros; simpl; auto.
+  intuition. subst; simpl in *.
+  pose proof (le_fold_max l v). omega.
+  simpl in *. eapply IHl; [ | eauto].
+  pose proof (le_fold_max_trans l (Peano.le_0_n a)).
+  omega.
+Qed.
+
+Definition keys T (l : VarMap.t T) := fst (split (VarMap.elements l)).
+
+Theorem varmap_find_oob : forall T (l : VarMap.t T) v,
+  v > list_max (keys l) ->
+  VarMap.find v l = None.
+Proof.
+  intros.
+  apply VarMapFacts.not_find_in_iff.
+  apply gt_list_max in H.
+  intuition.
+  apply H.
+  unfold keys. clear H; rename H0 into H.
+  apply VarMapFacts.elements_in_iff in H. destruct H.
+  erewrite <- ListUtils.fst_pair with (a := v).
+  apply in_split_l.
+  apply mapsto_elements.
+  apply VarMapFacts.elements_mapsto_iff.
+  all : eauto.
+Qed.
+
+Theorem vars_subset_refl :
+  forall V s, @vars_subset V s s.
+Proof.
+  unfold vars_subset.
+  eauto.
+Qed.
+
+Theorem vars_subset_trans :
+  forall V s1 s2 s3,
+    @vars_subset V s1 s2 ->
+    vars_subset s2 s3 ->
+    vars_subset s1 s3.
+Proof.
+  unfold vars_subset.
+  eauto.
+Qed.
+
+Hint Resolve vars_subset_refl vars_subset_trans.
+
+Lemma can_always_declare:
+  forall env t xp st,
+    exists st'' p'',
+      Go.step env (st, Go.Declare t xp) (st'', p'').
+Proof.
+  intros.
+  destruct_pair.
+  repeat eexists.
+  econstructor; eauto.
+  apply varmap_find_oob.
+  eauto.
+Qed.
+
+Local Open Scope map_scope.
+
+(* TODO: should have a more general way of dispatching goals like this *)
+Lemma subset_add_remove :
+  forall T var m m' (v : T),
+    vars_subset m' (var ->> v; m) ->
+    vars_subset (VarMap.remove var m') m.
+Proof.
+  unfold vars_subset; intros.
+  destruct (Nat.eq_dec k var).
+  - eauto using VarMapFacts.remove_eq_o.
+  - rewrite VarMapFacts.remove_neq_o; eauto.
+    eapply H.
+    rewrite VarMapFacts.add_neq_o; eauto.
+Qed.
+Hint Resolve subset_add_remove.
+
+Lemma subset_replace :
+  forall T var m (v0 v : T),
+    VarMap.find var m = Some v0 ->
+    vars_subset (var ->> v; m) m.
+Proof.
+  unfold vars_subset; intros.
+  destruct (Nat.eq_dec k var).
+  - congruence.
+  - rewrite VarMapFacts.add_neq_o; eauto.
+Qed.
+Hint Resolve subset_replace.
+
+Lemma subset_remove :
+  forall T var (m : VarMap.t T),
+    vars_subset (VarMap.remove var m) m.
+Proof.
+  unfold vars_subset; intros.
+  destruct (Nat.eq_dec k var).
+  - eauto using VarMapFacts.remove_eq_o.
+  - rewrite VarMapFacts.remove_neq_o; eauto.
+Qed.
+Hint Resolve subset_remove.
+
+Theorem exec_vars_decrease :
+  forall env p d d' s s',
+    Go.exec env ((d, s), p) (Go.Finished (d', s')) ->
+    vars_subset s' s.
+Proof.
+  intros.
+  find_eapply_lem_hyp Go.ExecFinished_Steps.
+  find_eapply_lem_hyp Go.Steps_runsto'.
+  prep_induction H; induction H; intros; subst; unfold Go.locals, Go.state in *;
+    repeat destruct_pair; repeat find_inversion_safe; eauto.
+    (* TODO: theorem about update_many *)
+    admit.
+  - subst_definitions.
+    admit. (* TODO: execution semantics are wrong here *)
+  - admit.
+Admitted.
+
+(* Something like this is true when [pr] does not fail:
+
+Theorem prog_vars_decrease :
+  forall T env A B p (pr : prog T),
+    EXTRACT pr
+    {{ A }}
+      p
+    {{ B }} // env ->
+    forall r,
+    match A, B r with
+      | Some A', Some B' => forall k, VarMap.In k B' -> VarMap.In k A'
+      | _, _ => True
+    end.
+Admitted.
+*)
+
+Lemma hoare_weaken_post : forall T env A (B1 B2 : T -> _) pr p,
+  (forall x, B1 x =p=> B2 x)%pred ->
+  EXTRACT pr
+  {{ A }} p {{ B1 }} // env ->
+  EXTRACT pr
+  {{ A }} p {{ B2 }} // env.
+Proof.
+  unfold ProgOk.
+  intros.
+  forwardauto H0.
+  intuition subst.
+  forwardauto H3; repeat deex;
+  repeat eexists; eauto.
+  unfold pred_apply in *.
+  pred_apply.
+  rewrite H.
+  eauto.
+  eauto.
+  eauto.
+Qed.
+
+Lemma hoare_strengthen_pre : forall T env A1 A2 (B : T -> _) pr p,
+  (A2 =p=> A1)%pred ->
+  EXTRACT pr
+  {{ A1 }} p {{ B }} // env ->
+  EXTRACT pr
+  {{ A2 }} p {{ B }} // env.
+Proof.
+  unfold ProgOk, pred_apply in *; intros.
+  apply H in H1.
+  forward_solve.
+Qed.
+
+Lemma hoare_weaken : forall T env A1 A2 (B1 B2 : T -> _) pr p,
+  EXTRACT pr
+  {{ A1 }} p {{ B1 }} // env ->
+  (A2 =p=> A1)%pred ->
+  (forall x, B1 x =p=> B2 x)%pred ->
+  EXTRACT pr
+  {{ A2 }} p {{ B2 }} // env.
+Proof.
+  eauto using hoare_strengthen_pre, hoare_weaken_post.
+Qed.
+
+Instance progok_hoare_proper :
+  forall T env pr,
+  Proper (@prog_equiv T ==> Basics.flip pimpl ==> pointwise_relation _ pimpl ==> Basics.impl) (@ProgOk T env pr).
+Proof.
+  intros.
+  intros pr1 pr2 Hpr A1 A2 Hpre B1 B2 Hpost H.
+  eauto using hoare_strengthen_pre, hoare_weaken_post, extract_equiv_prog.
+Qed.
+
+Instance piff_progok_proper : forall T p xp env,
+  Proper (piff ==> pointwise_relation T piff ==> flip Basics.impl) (ProgOk env p xp).
+Proof.
+  repeat intro.
+  rewrite H in H2.
+  setoid_rewrite H0.
+  unshelve (edestruct H1); eauto.
+Defined.
+
+(*
+Theorem extract_finish_equiv : forall A {H: GoWrapper A} scope cscope pr p,
+  (forall d0,
+    {{ SItemDisk (NTSome "disk") d0 (ret tt) :: scope }}
+      p
+    {{ [ SItemDisk (NTSome "disk") d0 pr; SItemRet (NTSome "out") d0 pr ] }} {{ cscope }} // disk_env) ->
+  forall st st' d0,
+    st ## ( SItemDisk (NTSome "disk") d0 (ret tt) :: scope) ->
+    RunsTo disk_env p st st' ->
+    exists d', find "disk" st' = Some (Disk d') /\ exists r, @computes_to A pr d0 d' r.
+Proof.
+  unfold ProgOk.
+  intros.
+  specialize (H0 d0 st ltac:(auto)).
+  intuition.
+  specialize (H5 st' ltac:(auto)).
+  simpl in *.
+  find_cases "disk" st.
+  find_cases "disk" st'.
+  intuition.
+  repeat deex.
+  intuition eauto.
+Qed.
+
+Theorem extract_crash_equiv : forall A pscope scope pr p,
+  (forall d0,
+    {{ SItemDisk (NTSome "disk") d0 (ret tt) :: scope }}
+      p
+    {{ pscope }} {{ [ SItemDiskCrash (NTSome "disk") d0 pr ] }} // disk_env) ->
+  forall st p' st' d0,
+    st ## (SItemDisk (NTSome "disk") d0 (ret tt) :: scope) ->
+    (Go.step disk_env)^* (p, st) (p', st') ->
+    exists d', find "disk" st' = Some (Disk d') /\ @computes_to_crash A pr d0 d'.
+Proof.
+  unfold ProgOk.
+  intros.
+  specialize (H d0 st ltac:(auto)).
+  intuition.
+  specialize (H st' p').
+  simpl in *.
+  intuition. find_cases "disk" st'.
+  repeat deex. eauto.
+Qed.
+*)
