src/GoHoare.v
@@ -1,0 +1,257 @@
+Require Import FunctionalExtensionality ProofIrrelevance.
+Require Import PeanoNat List Structures.OrderedTypeEx.
+Require Import RelationClasses Morphisms.
+Require Import VerdiTactics GoTactics1.
+Require Import GoSemantics.
+Require Import Word Prog ProgMonad Pred AsyncDisk.
+
+Set Implicit Arguments.
+Unset Printing Implicit Defensive.
+
+Class GoWrapper (WrappedType: Type) :=
+  {
+    wrap_type: Go.type;
+    wrap':     WrappedType -> Go.type_denote wrap_type;
+    wrap_inj:  forall a1 a2, wrap' a1 = wrap' a2 -> a1 = a2;
+  }.
+
+Definition wrap T {Wr: GoWrapper T} (t : T) : Go.value := Go.Val wrap_type (wrap' t).
+
+Definition pred := @Pred.pred Go.var Nat.eq_dec Go.value.
+
+Notation "k ~> v" := (k |-> (wrap v))%pred (at level 35) : pred_scope.
+
+Definition mem_of := ((fun m k => VarMap.find k m) : Go.locals -> @Mem.mem Go.var Nat.eq_dec Go.value).
+
+Notation "m ≲ p" := (mem_of m ## p) (at level 70).
+
+
+Notation "k ~>? T" := (exists val, k |-> Go.Val (@wrap_type T _) val)%pred (at level 35) : pred_scope.
+
+Definition ProgOk T env eprog (sprog : prog T) (initial_tstate : pred) (final_tstate : T -> pred) :=
+  forall initial_state hm,
+    (snd initial_state) ≲ initial_tstate ->
+    forall out,
+      Go.exec env (initial_state, eprog) out ->
+    (forall final_state, out = Go.Finished final_state ->
+      exists r hm',
+        exec (fst initial_state) hm sprog (Finished (fst final_state) hm' r) /\
+        (snd final_state ≲ final_tstate r)) /\
+    (forall final_disk,
+      out = Go.Crashed final_disk ->
+      exists hm',
+        exec (fst initial_state) hm sprog (Crashed T final_disk hm')) /\
+    (out = Go.Failed ->
+      exec (fst initial_state) hm sprog (Failed T)).
+
+Notation "'EXTRACT' SP {{ A }} EP {{ B }} // EV" :=
+  (ProgOk EV EP%go SP A%pred B%pred)
+    (at level 60, format "'[v' 'EXTRACT'  SP '/' '{{'  A  '}}' '/'    EP '/' '{{'  B  '}}'  //  EV ']'").
+
+
+Create HintDb gowrapper discriminated.
+
+Hint Resolve wrap_inj : gowrapper.
+
+Ltac GoWrapper_finish :=
+  solve [simpl; (f_equal + idtac); eauto using inj_pair2 with gowrapper].
+
+Ltac GoWrapper_t :=
+  abstract (repeat match goal with
+                   | _ => progress intros
+                   | _ => progress (repeat find_inversion_safe)
+                   | [ H : unit |- _ ] => destruct H
+                   | [ H : _ * _ |- _ ] => destruct H
+                   | _ => GoWrapper_finish
+                   end).
+
+Instance GoWrapper_Num : GoWrapper W.
+Proof.
+  refine {| wrap' := Go.Here;
+            wrap_type := Go.Num |}; GoWrapper_t.
+Defined.
+
+Instance GoWrapper_Bool : GoWrapper bool.
+Proof.
+  refine {| wrap' := id;
+            wrap_type := Go.Bool |}; GoWrapper_t.
+Defined.
+
+Instance GoWrapper_valu : GoWrapper valu.
+Proof.
+  refine {| wrap' := Go.Here;
+            wrap_type := Go.DiskBlock |}; GoWrapper_t.
+Defined.
+
+Instance GoWrapper_unit : GoWrapper unit.
+Proof.
+  refine {| wrap' := id;
+            wrap_type := Go.EmptyStruct |}; GoWrapper_t.
+Defined.
+
+Instance GoWrapper_pair {A B} {WA : GoWrapper A} {WB : GoWrapper B} : GoWrapper (A * B).
+Proof.
+  refine {| wrap' := fun p => (wrap' (fst p), wrap' (snd p));
+            wrap_type := Go.Pair (@wrap_type _ WA) (@wrap_type _ WB) |}; GoWrapper_t.
+Defined.
+
+Lemma map_inj_inj :
+  forall A B (f : A -> B),
+    (forall a1 a2, f a1 = f a2 -> a1 = a2) ->
+    forall as1 as2,
+      map f as1 = map f as2 ->
+      as1 = as2.
+Proof.
+  induction as1; intros; destruct as2; simpl in *; try discriminate; auto.
+  find_inversion.
+  f_equal; eauto.
+Qed.
+Hint Resolve map_inj_inj : gowrapper.
+
+Instance GoWrapper_list T {Wr: GoWrapper T} : GoWrapper (list T).
+Proof.
+  refine {| wrap' := fun l => Go.Here (map wrap' l);
+            wrap_type := Go.Slice wrap_type |}; GoWrapper_t.
+Defined.
+
+Instance GoWrapper_option {A} {WA : GoWrapper A} : GoWrapper (option A).
+Proof.
+  refine {| wrap' := fun o => match o with
+                              | None => (false, Go.default_value' _)
+                              | Some x => (true, wrap' x) end;
+            wrap_type := Go.Pair Go.Bool (@wrap_type _ WA)|}.
+  intros a b H.
+  destruct a, b; invc H; GoWrapper_t.
+Defined.
+
+Instance GoWrapper_dec {P Q} : GoWrapper ({P} + {Q}).
+Proof.
+  refine {| wrap' := fun (v : {P} + {Q}) => if v then true else false;
+            wrap_type := Go.Bool |}.
+  intros.
+  destruct a1, a2; f_equal; try discriminate; apply proof_irrelevance.
+Qed.
+
+
+Instance GoWrapper_addrmap {T} {WT : GoWrapper T} : GoWrapper (Go.Map.t T).
+Proof.
+  refine {| wrap_type := Go.AddrMap (@wrap_type _ WT);
+            wrap' := fun m => Go.Here (Go.Map.map (@wrap' _ WT) m) |}.
+  intros.
+  apply MapUtils.addrmap_equal_eq.
+  pose proof (MapUtils.AddrMap.MapFacts.Equal_refl
+    (Go.Map.map wrap' a1)) as H0.
+  find_inversion_go. rewrite H in H0 at 2.
+  eapply MoreAddrMapFacts.map_inj_equal; eauto.
+  exact (@wrap_inj _ WT).
+Defined.
+
+Class DefaultValue T {Wrapper : GoWrapper T} :=
+  {
+    zeroval : T;
+    default_zero : wrap zeroval = Go.default_value wrap_type;
+  }.
+
+Arguments DefaultValue T {Wrapper}.
+
+Instance num_default_value : DefaultValue nat := {| zeroval := 0 |}. auto. Defined.
+Instance valu_default_value : DefaultValue valu := {| zeroval := $0 |}. auto. Defined.
+Instance bool_default_value : DefaultValue bool := {| zeroval := false |}. auto. Defined.
+Instance emptystruct_default_value : DefaultValue unit := {| zeroval := tt |}. auto. Defined.
+
+Instance option_default_value T {H : GoWrapper T} : DefaultValue (option T) := {| zeroval := None |}. auto. Defined.
+
+Import Go ListNotations.
+
+Lemma default_zero' :
+  forall T {W : GoWrapper T} v,
+    wrap v = default_value wrap_type -> wrap' v = default_value' wrap_type.
+Proof.
+  unfold wrap, default_value; intros.
+  eauto using value_inj.
+Qed.
+
+Instance pair_default_value A B {Wa : GoWrapper A} {Wb : GoWrapper B}
+  {Da : DefaultValue A} {Db : DefaultValue B} : DefaultValue (A * B) := {| zeroval := (zeroval, zeroval) |}.
+  destruct Da, Db. unfold wrap; simpl. repeat find_apply_lem_hyp default_zero'.
+  repeat find_rewrite. reflexivity.
+Defined.
+
+Instance list_default_value A {W : GoWrapper A} : DefaultValue (list A) := {| zeroval := [] |}. auto. Defined.
+
+Class WrapByTransforming T := {
+  T' : Type;
+  WrT' : GoWrapper T';
+  transform : T -> T';
+  transform_inj : forall t1 t2 : T, transform t1 = transform t2 -> t1 = t2;
+}.
+
+Instance GoWrapper_transform T {Tr : WrapByTransforming T} : GoWrapper T.
+  refine {| wrap_type := wrap_type;
+            wrap' := fun t => @wrap' _ (@WrT' _ Tr) (@transform _ Tr t) |}.
+  intros.
+  apply wrap_inj in H.
+  auto using transform_inj.
+Defined.
+
+
+Theorem transform_pimpl : forall T {Tr : WrapByTransforming T} k (t : T),
+  (k |-> (@wrap _ (@GoWrapper_transform _ Tr) t) : pred) <=p=> k |-> (@wrap _ WrT' (transform t)).
+Proof.
+  intros.
+  reflexivity.
+Qed.
+
+
+Lemma extract_equiv_prog : forall T env A (B : T -> _) pr1 pr2 p,
+  prog_equiv pr1 pr2 ->
+  EXTRACT pr1
+  {{ A }}
+    p
+  {{ B }} // env ->
+  EXTRACT pr2
+  {{ A }}
+    p
+  {{ B }} // env.
+Proof.
+  unfold prog_equiv, ProgOk.
+  intros.
+  setoid_rewrite <- H.
+  auto.
+Qed.
+
+
+Module VarMapFacts := FMapFacts.WFacts_fun(Nat_as_OT)(VarMap).
+
+Theorem add_upd :
+  forall m k v,
+    mem_of (VarMap.add k v m) = Mem.upd (mem_of m) k v.
+Proof.
+  intros.
+  extensionality k0.
+  unfold mem_of, Mem.upd.
+  rewrite VarMapFacts.add_o.
+  repeat break_match; congruence.
+Qed.
+
+Theorem remove_delete :
+  forall m k,
+    mem_of (VarMap.remove k m) = Mem.delete (mem_of m) k.
+Proof.
+  intros.
+  extensionality k0.
+  unfold mem_of, Mem.delete.
+  rewrite VarMapFacts.remove_o.
+  repeat break_match; congruence.
+Qed.
+
+Fact sep_star_ptsto_some_find : forall l var val A,
+  l ≲ (var |-> val * A) -> VarMap.find var l = Some val.
+Proof.
+  intros.
+  find_eapply_lem_hyp sep_star_ptsto_some.
+  eauto.
+Qed.
+
+Hint Resolve sep_star_ptsto_some_find. (* TODO hintdb *)
+
