src/GoTactics1.v
@@ -1,0 +1,71 @@
+Require Export VerdiTactics.
+Require Import Pred Hoare.
+Require Import SepAuto.
+Require Import GoSemantics.
+
+Ltac set_hyp_evars :=
+  repeat match goal with
+  | [ H : context[?e] |- _ ] =>
+    is_evar e;
+    let H := fresh in
+    set (H := e) in *
+  end.
+
+Ltac invert_trivial H :=
+  match type of H with
+    | ?con ?a = ?con ?b =>
+      let H' := fresh in
+      assert (a = b) as H' by exact (match H with eq_refl => eq_refl end); clear H; rename H' into H
+  end.
+
+
+Lemma pair_inj :
+  forall A B (a1 a2 : A) (b1 b2 : B), (a1, b1) = (a2, b2) -> a1 = a2 /\ b1 = b2.
+Proof.
+  intros. find_inversion. auto.
+Qed.
+
+
+Lemma some_inj :
+  forall A (x y : A), Some x = Some y -> x = y.
+Proof.
+  intros. find_inversion. auto.
+Qed.
+
+Lemma Val_type_inj :
+  forall t1 t2 v1 v2, Go.Val t1 v1 = Go.Val t2 v2 -> t1 = t2.
+Proof.
+  intros. find_inversion. auto.
+Qed.
+
+Lemma Here_inj :
+  forall T (a b : T), Go.Here a = Go.Here b -> a = b.
+Proof.
+  intros. find_inversion. auto.
+Qed.
+
+Ltac find_inversion_safe :=
+  match goal with
+  | [ H : ?X ?a = ?X ?b |- _ ] =>
+    (unify a b; fail 1) ||
+    let He := fresh in
+    assert (a = b) as He by solve [inversion H; auto with equalities | invert_trivial H; auto with equalities]; clear H; subst
+  | [ H : ?X ?a1 ?a2 = ?X ?b1 ?b2 |- _ ] =>
+    (unify a1 b1; unify a2 b2; fail 1) ||
+    let He := fresh in
+    assert (a1 = b1 /\ a2 = b2) as He by solve [inversion H; auto with equalities | invert_trivial H; auto with equalities]; clear H; destruct He as [? ?]; subst
+  | [ H : (?a, ?b) = (?c, ?d) |- _ ] =>
+    apply pair_inj in H; destruct H; try (subst a || subst c); try (subst b || subst d)
+  end.
+
+Ltac find_inversion_go :=
+  match goal with
+  | [ H : Some ?x = Some ?y |- _ ] => apply some_inj in H; try (subst x || subst y)
+  | [ H : Go.Val ?ta ?a = Go.Val ?tb ?b |- _ ] =>
+    (unify ta tb; unify a b; fail 1) ||
+    assert (ta = tb) by (eapply Val_type_inj; eauto); try (subst ta || subst tb);
+    assert (a = b) by (eapply Go.value_inj; eauto); clear H; try (subst a || subst b)
+  | [ H : Go.Here ?a = Go.Here ?b |- _ ] =>
+    apply Here_inj in H; try (subst a || subst b)
+  | _ => find_inversion_safe
+  end.
