src/GoTactics2.v
@@ -1,0 +1,270 @@
+Require Import ProofIrrelevance Eqdep_dec.
+Require Import Omega VerdiTactics.
+Require Import Mem Pred Hoare.
+Require Import SepAuto.
+Require Import GoSemantics GoHoare.
+Require Export GoTactics1.
+
+
+Local Open Scope string_scope.
+
+Ltac find_cases var st := case_eq (VarMap.find var st); [
+  let v := fresh "v" in
+  let He := fresh "He" in
+  intros v He; rewrite ?He in *
+| let Hne := fresh "Hne" in
+  intro Hne; rewrite Hne in *; exfalso; solve [ discriminate || intuition idtac ] ].
+
+
+Ltac inv_exec :=
+  match goal with
+  | [ H : Go.step _ _ _ |- _ ] => invc H
+  | [ H : Go.exec _ _ _ |- _ ] => invc H
+  | [ H : Go.crash_step _ |- _ ] => invc H
+  end; try discriminate.
+
+
+Theorem eq_dec_eq :
+  forall A (dec : forall a1 a2 : A, {a1 = a2} + {a1 <> a2}) a,
+    dec a a = left eq_refl.
+Proof.
+  intros.
+  destruct (dec a a); try congruence.
+  f_equal.
+  apply UIP_dec; assumption.
+Qed.
+
+Ltac forwardauto1 H :=
+  repeat eforward H; conclude H eauto.
+
+Ltac forwardauto H :=
+  forwardauto1 H; repeat forwardauto1 H.
+
+Ltac forward_solve_step :=
+  match goal with
+    | _ => progress intuition eauto
+    | [ H : forall _, _ |- _ ] => forwardauto H
+    | _ => deex
+    | _ => discriminate
+  end.
+
+Ltac forward_solve :=
+  repeat forward_solve_step.
+
+Import Go.
+
+Ltac unfold_expr :=
+  match goal with
+  | [H : _ |- _ ] =>
+      progress (unfold is_false, is_true, eval_bool,
+         numop_impl', numop_impl,
+         split_pair_impl, split_pair_impl',
+         join_pair_impl, join_pair_impl',
+         map_add_impl, map_add_impl',
+         map_remove_impl, map_remove_impl',
+         map_find_impl, map_find_impl',
+         map_card_impl, map_card_impl',
+         map_elements_impl, map_elements_impl',
+         eval_test_m, eval_test_num, eval_test_bool,
+         update_one, setconst_impl, duplicate_impl,
+         sel, id, eval, eq_rect_r, eq_rect
+         in H); simpl in H
+  | _ => progress (unfold is_false, is_true, eval_bool,
+         numop_impl', numop_impl,
+         split_pair_impl, split_pair_impl',
+         join_pair_impl, join_pair_impl',
+         map_add_impl, map_add_impl',
+         map_remove_impl, map_remove_impl',
+         map_find_impl, map_find_impl',
+         map_card_impl, map_card_impl',
+         map_elements_impl, map_elements_impl',
+         eval_test_m, eval_test_num, eval_test_bool,
+         update_one, setconst_impl, duplicate_impl,
+         sel, id, eval, eq_rect_r, eq_rect
+         ); simpl
+  end.
+
+
+Ltac deex_hyp H :=
+  match type of H with
+  | exists varname, _ =>
+    let varname' := fresh varname in
+    destruct H as (varname', H); intuition subst
+  end.
+
+
+Ltac find_inversion_wrap :=
+  match goal with
+    | [ H : wrap _ = Go.Val _ _ |- _ ] => unfold wrap in H; simpl in H; unfold id in H
+    | [ H : Go.Val _ _ = wrap _ |- _ ] => unfold wrap in H; simpl in H; unfold id in H
+    | _ => find_inversion_go
+  end.
+
+Ltac match_finds :=
+  match goal with
+    | [ H1: VarMap.find ?a ?s = ?v1, H2: VarMap.find ?a ?s = ?v2 |- _ ] => rewrite H1 in H2;
+      (find_inversion_wrap || invc H2 || idtac)
+  end.
+
+Ltac destruct_pair :=
+  match goal with
+    | [ H : _ * _ |- _ ] => destruct H
+    | [ H : Go.state |- _ ] => destruct H
+  end.
+
+Ltac inv_exec_progok :=
+  repeat destruct_pair; repeat inv_exec; unfold Go.sel in *; simpl in *;
+  intuition (subst; try discriminate;
+             repeat find_inversion_safe; repeat match_finds; repeat find_inversion_safe;  simpl in *;
+               try solve [ exfalso; intuition eauto 10 ]; eauto 10).
+
+Ltac extract_var_val_from H P s :=
+  match P with
+  | context[(?a |-> ?v)%pred] =>
+    match goal with
+    | [ H: VarMap.find a s = Some v |- _ ] => fail 1
+    | _ => idtac
+    end;
+    let He := fresh "He" in
+    assert (VarMap.find a s = Some v) as He; [
+      eapply pred_apply_pimpl_proper in H; [
+      | reflexivity |
+      lazymatch goal with
+      | [ |- _ =p=> ?Q ] =>
+        let F := fresh "F" in
+        evar (F : pred);
+        unify Q (a |-> v * F)%pred;
+        cancel
+      end ];
+      eapply ptsto_valid in H; eassumption
+    | try rewrite He in * ]
+  end.
+
+Ltac extract_var_val :=
+  lazymatch goal with
+  | [ H: ?s ≲ ?P |- _ ] => extract_var_val_from H P s
+  | [ H: (?P)%pred (mem_of ?s) |- _ ] => extract_var_val_from H P s
+  end.
+
+Ltac extract_pred_apply_exists :=
+  match goal with
+  | [ H : _ ≲ _ |- _ ] =>
+    repeat setoid_rewrite pimpl_exists_l_star_r in H;
+    repeat setoid_rewrite pimpl_exists_r_star_r in H;
+      unfold pred_apply, exis in H; deex_hyp H; repeat deex_hyp H
+  end.
+
+Ltac eval_expr_step :=
+    repeat extract_var_val;
+    repeat (destruct_pair + unfold_expr); simpl in *;
+    try extract_pred_apply_exists;
+    try subst;
+    match goal with
+    | [H : context [match ?e in (_ = _) return _ with _ => _ end] |- _ ]
+      => rewrite (proof_irrelevance _ e (eq_refl)) in H
+    | [H : context [eq_sym ?t] |- _ ]
+      => setoid_rewrite (proof_irrelevance _ t eq_refl) in H
+    | [e : ?x = _, H: context[match ?x with _ => _ end] |- _]
+      => rewrite e in H
+    | [e : ?x = _ |- context[match ?x with _ => _ end] ]
+      => rewrite e
+    | [H : context[if ?x then _ else _] |- _]
+      => let H' := fresh in destruct x eqn:H'; try omega
+    | [|- context[if ?x then _ else _] ]
+      => let H' := fresh in destruct x eqn:H'; try omega
+    | [H : context [match ?x with _ => _ end],
+       H': _ = ?x |- _]
+      => rewrite <- H' in H
+    | [H : context [match ?x with _ => _ end],
+       H': ?x = _ |- _]
+      => rewrite H' in H
+    | [H : context [match ?x with _ => _ end] |- _]
+      => let H' := fresh in destruct x eqn:H'
+    | [ |- context [match ?e in (_ = _) return _ with _ => _ end] ]
+      => rewrite (proof_irrelevance _ e (eq_refl))
+    | [ |- context [eq_sym ?t] ]
+      => setoid_rewrite (proof_irrelevance _ t eq_refl)
+    | [ |- context [match ?x with _ => _ end] ]
+      => let H' := fresh in destruct x eqn:H'
+    | _
+      => idtac
+    end; try solve [congruence | omega];
+    repeat find_inversion_wrap.
+
+Ltac eval_expr := repeat eval_expr_step.
+
+
+Definition prod' := prod.
+Definition exis' := exis.
+
+Hint Extern 0 (okToUnify (ptsto ?a _) (ptsto ?b _)) => unify a b; reflexivity : okToUnify.
+
+
+Lemma ptsto_upd_disjoint' : forall (F : pred) a v m,
+  F m -> m a = None
+  -> (a |-> v * F)%pred (upd m a v).
+Proof.
+  intros.
+  eapply pred_apply_pimpl_proper; [ reflexivity | | eapply ptsto_upd_disjoint; eauto ].
+  cancel.
+Qed.
+
+Create HintDb cancel_go_finish.
+
+Ltac cancel_go :=
+  simpl in *;
+  fold prod' in *; fold exis' in *;
+  cancel;
+  (solve [
+    match goal with
+      | [ |- (?P =p=> ?Q)] =>
+      set (H := Q);
+      unfold exis' in H; subst H; cancel
+    end; cancel |
+    unfold exis'; cancel; auto with cancel_go_finish ])
+    || cancel.
+
+Lemma ptsto_delete' : forall a (F :pred) (m : mem),
+  (a |->? * F)%pred m -> F (delete m a).
+Proof.
+  intros.
+  apply pimpl_exists_r_star_r in H.
+  unfold exis in H.
+  deex.
+  eapply ptsto_delete; eauto.
+Qed.
+
+Ltac pred_solve_step := match goal with
+  | [ |- ( ?P )%pred (upd _ ?a ?x) ] =>
+    match P with
+    | context [(a |-> ?x)%pred] =>
+      eapply pimpl_apply with (p := (a |-> x * _)%pred);
+      [ cancel_go | (eapply ptsto_upd_disjoint'; solve [eauto]) || eapply ptsto_upd ]
+    | context [(@ptsto ?AT ?AEQ ?V a ?y)%pred] =>
+      let H := fresh in
+      assert (@okToUnify AT AEQ V (ptsto a y) (ptsto a x)) as H;
+      [ eauto with okToUnify | rewrite H ]
+    end
+  | [ |- ( ?P )%pred (delete _ ?a) ] =>
+    eapply ptsto_delete' with (F := P)
+  | [ H : _%pred ?t |- _%pred ?t ] => pred_apply; solve [cancel_go]
+  | _ => solve [cancel_go]
+  end.
+
+Create HintDb pred_solve_rewrites.
+Hint Rewrite add_upd remove_delete : pred_solve_rewrites.
+(* Coq bug! This hangs:
+Hint Rewrite default_zero : pred_solve_rewrites.
+*)
+
+Ltac pred_solve := progress (
+  unfold pred_apply in *;
+  repeat pred_solve_step;
+  repeat (autorewrite with pred_solve_rewrites || rewrite ?default_zero);
+  repeat pred_solve_step).
+
+Ltac pred_cancel :=
+  unfold pred_apply in *;
+  match goal with
+  | [H : _ |- _] => eapply pimpl_apply; [> | exact H]; solve [cancel_go]
+  end.
